SSGpd: the construction of semi-simplicial groupoids (#23)
# `SSGpd`: the construction of semi-simplicial groupoids

### About the construction

- we replace h-sets with h-groupoids
- we fix the arity to `n = 1`, the simplicial case (for simplicity)
- we add a third mutual recursion block: the proof of `mkCohFrames` is
done together with `mkCoh2FrameTypes`
- we prove 2-level coherences: `mkCoh2Frames`, `mkCoh2Layer`,
`mkCoh2Paintings`
- 3-level frame coherence is closed by `GUIP`, groupoid's path `UIP`
assumption

### What makes it all possible

The observation: the structure of coherence proofs is the same, not just
across different coherences (`νDgnSet` coherences follow the same
structure as `νSet` one), but also across different coherence levels.

- frame coherence induction: decomposition into a proof of frame
coherence (recursively) and a proof of layer coherence
- level one is done by `eq_existT_curried`, level two is done by
`eq_existT_curried_hex`
- layer coherence: decomposition into a proof of painting coherence,
plus a proof of frame coherence *one level up*
- level one is done by `rew_cohLayer`, level two by `rew_coh2Layer`
- painting coherence induction: decomposition into a proof of layer
coherence and a proof of painting coherence (recursively)
- level one is done by `eq_existT_curried_dep`, level two is done by
`eq_existT_curried_dep_hex`

### Glue - the `SSGpdLemmas` file

These lemmas abstract away the frame/layer/painting structure of the
construction, and encapsulate all of the path algebra we need for
coherence proofs.

`eq_existT_curried_hex` - the 2-level analogue of `eq_existT_curried`
used in `mkCoh2Frames`, fuses 3 things:
- `f_equal_eq_existT_curried` - `eq_existT_curried` commutes with
`f_equal`
- `eq_trans_eq_existT_curried` - `eq_existT_curried` commutes with
`eq_trans`
- `eq_existT_curried_eq` - assembles an equality of paths built with
`eq_existT_curried`

`eq_existT_curried_dep_hex` - 2-level analogue of
`eq_existT_curried_dep`, used in induction step case of `mkCoh2Painting`

`rew_cohLayer` - a single lemma that fuses the entire rewrite chain of
the layer coherence proof:
- a couple of `map_subst` rewrites
- multiple `rew_map` rewrites
- multiple `rew_compose` rewrites
- a `rew_swap` application
- a rewrite with `rew_app_rl`

`rew_coh2Layer` - a 2-level analogue of `rew_cohLayer`, encapsulates all
of the path algebra needed for `mkCoh2Layer` proof

`permutahedral_coherence` - a helper definition for `rew_coh2Layer`

`rew_coh2Painting_restr0` - a lemma for the base case of
`mkCoh2Painting`. Unlike the 1-level case, it doesn't hold by
`reflexivity`

### Outcome

The `SemiSimplicial5` example, as computed in `νSet` from the
`no-funext` branch, gets stuck on h-set's `UIP`. In contrast, in
`SSGpd`, `SemiSimplicial5` fully computes. `SemiSimplicial6` gets stuck
on `GUIP`, groupoid's `UIP`.

### Compilation performance

There were a few issues to overcome. It is recommended to use
[master+bonak-patches](https://github.com/olympichek/rocq/tree/master%2Bbonak-patches)
branch to compile this project. With this branch the project compiles in
1m 20s on my laptop.

This branch contains:
- Pierre-Marie Pédrot's fixpoint refolding patches
- A patch to make `whd_all` and `whd_allnolet` go through `CClosure`, to
benefit from fixpoint refolding
- A fast path in conversion's `compare_under` (now merged as
[#22299](https://github.com/rocq-prover/rocq/pull/22299))
- An implementation of cache for Rocq's conversion

### Future work: going back to abstract arity

This is a follow-up step, still an open problem.

Both known approaches have issues:
- layers as functions from arity: layer coherence proofs don't compute,
get stuck on fun-ext axiom
- layers as vectors: require more rewrites, complicate 2-level proofs,
harder to abstract

### Future work: helper lemmas in a stronger type theory

Investigate whether at least some of the lemmas from `SSGpdLemmas` are
true by definition in a type theory with more definitional rules, such
as Cubical Type Theory or Higher Observational Type Theory. Definitional
rule establishing that equality of pairs is a pair of equality proofs by
definition seems to be particularly useful here.

### Future work: towards infinity

Now we just need to understand how to generalize the coherence proof
pattern from sets and groupoids to n-groupoids and ∞-groupoids..

theories/νSet/SigT.v
@@ -60,4 +60,170 @@ Lemma eq_existT_curried_dep {A x} {P: A -> Type} {Q: {a &T P a} -> Type}
    rew [fun x => {a: P x &T Q (x; a)}] H in (u; v) = (u'; v').
 Proof.
    now destruct Hu, Hv, H.
-Qed.
+Defined.
+
+Lemma eq_existT_curried_eq {A: Type} {P: A -> Type}
+  {x y: A} {u: P x} {v: P y}
+  {p p': x = y}
+  {q: rew [P] p in u = v} {q': rew [P] p' in u = v}
+  (Hp: p = p')
+  (Hq: rew [fun r => rew [P] r in u = v] Hp in q = q'):
+  (= p; q) = (= p'; q').
+Proof.
+  destruct Hp; simpl in Hq. now destruct Hq.
+Defined.
+
+Lemma eq_existT_curried_dep_eq {A x y} {P: A -> Type}
+  {Q: {a &T P a} -> Type}
+  {H H': x = y}
+  {u: P x} {v: Q (x; u)}
+  {u': P y} {v': Q (y; u')}
+  {Hu: rew [P] H in u = u'} {Hu': rew [P] H' in u = u'}
+  {Hv: rew [Q] (=H; Hu) in v = v'}
+  {Hv': rew [Q] (=H'; Hu') in v = v'}
+  (HH: H = H')
+  (HHu: rew [fun H => rew [P] H in u = u'] HH in Hu = Hu')
+  (HHv: rew [fun p => rew [Q] p in v = v']
+    eq_existT_curried_eq HH HHu in Hv = Hv'):
+  rew [fun H => rew [fun x => {a: P x &T Q (x; a)}] H in
+    (u; v) = (u'; v')] HH in
+  @eq_existT_curried_dep A x P Q y H u v u' v' Hu Hv =
+  @eq_existT_curried_dep A x P Q y H' u v u' v' Hu' Hv'.
+Proof.
+  destruct HH; cbn in HHu. destruct HHu; cbn in HHv.
+  now destruct HHv.
+Defined.
+
+Definition sigT_map_eq {A B: Type} {P: A -> Type} {Q: B -> Type}
+  {f: A -> B} (g: forall a, P a -> Q (f a))
+  {x y: A} {u: P x} {v: P y}
+  {p: x = y} (q: rew [P] p in u = v):
+  rew [Q] f_equal f p in g x u = g y v.
+Proof.
+  now destruct q, p.
+Defined.
+
+Lemma sigT_map_eq_id_refl {A B: Type} {Q: B -> Type} (f: A -> B)
+  {x: A} {u v: Q (f x)} (q: u = v):
+  @sigT_map_eq A B (fun a => Q (f a)) Q f (fun a u => u) x x u v eq_refl q = q.
+Proof.
+  now destruct q.
+Defined.
+
+Lemma sigT_map_eq_refl {A B: Type} {P: A -> Type} {Q: B -> Type}
+  {f: A -> B} (g: forall a, P a -> Q (f a))
+  {x: A} {u v: P x} (q: u = v):
+  sigT_map_eq g (p := eq_refl) q = f_equal (g x) q.
+Proof.
+  now destruct q.
+Defined.
+
+Lemma f_equal_eq_existT_curried {A B: Type} {P: A -> Type} {Q: B -> Type}
+  (f: A -> B) (g: forall a, P a -> Q (f a))
+  {x y: A} {u: P x} {v: P y}
+  (p: x = y) (q: rew [P] p in u = v):
+  f_equal (fun z: {a: A &T P a} => (f z.1; g z.1 z.2)) (= p; q) =
+  (= f_equal f p; sigT_map_eq g q).
+Proof.
+  now destruct q, p.
+Defined.
+
+Lemma sigT_map_eq_existT_curried_dep_fst {A B: Type} {P: A -> Type}
+  {P': B -> Type} {Q: {a: A &T P a} -> Type}
+  (f: A -> B) (g: forall a, P a -> P' (f a))
+  {x y: A} {u: P x} {v: Q (x; u)}
+  {u': P y} {v': Q (y; u')}
+  (H: x = y) (Hu: rew [P] H in u = u')
+  (Hv: rew [Q] (=H; Hu) in v = v'):
+  sigT_map_eq
+    (P := fun a => {u: P a &T Q (a; u)})
+    (Q := P')
+    (fun a uv => g a uv.1)
+    (eq_existT_curried_dep (H := H) (Hu := Hu) (Hv := Hv)) =
+  sigT_map_eq g Hu.
+Proof.
+  now destruct Hv, Hu, H.
+Defined.
+
+Lemma sigT_map_eq_existT_curried_dep_curried {A B: Type} {P: A -> Type}
+  {R: forall a, P a -> Type} {P': B -> Type}
+  {R': forall b, P' b -> Type}
+  (f: A -> B) (g: forall a, P a -> P' (f a))
+  (h: forall a u, R a u -> R' (f a) (g a u))
+  {x y: A} {u: P x} {v: R x u}
+  {u': P y} {v': R y u'}
+  (H: x = y) (Hu: rew [P] H in u = u')
+  (Hv: rew [fun z => R z.1 z.2] (=H; Hu) in
+    (v: (fun z => R z.1 z.2) (x; u)) = v'):
+  sigT_map_eq
+    (P := fun a => {u: P a &T R a u})
+    (Q := fun b => {u: P' b &T R' b u})
+    (fun a uv => (g a uv.1; h a uv.1 uv.2))
+    (eq_existT_curried_dep (Q := fun z => R z.1 z.2)
+      (H := H) (Hu := Hu) (Hv := Hv)) =
+  eq_existT_curried_dep
+    (Q := fun z => R' z.1 z.2)
+    (H := f_equal f H)
+    (Hu := sigT_map_eq g Hu)
+    (Hv := rew [fun p => rew [fun z => R' z.1 z.2] p in
+        (h x u v: (fun z => R' z.1 z.2) (f x; g x u)) =
+        (h y u' v': (fun z => R' z.1 z.2) (f y; g y u'))]
+      f_equal_eq_existT_curried f g H Hu in
+      @sigT_map_eq _ _ (fun z => R z.1 z.2) (fun z => R' z.1 z.2)
+        (fun z => (f z.1; g z.1 z.2))
+        (fun z => h z.1 z.2) (x; u) (y; u') v v' (=H; Hu) Hv).
+Proof.
+  now destruct Hv, Hu, H.
+Defined.
+
+Definition sigT_trans_eq {A: Type} {P: A -> Type}
+  {x y z: A} {u: P x} {v: P y} {w: P z}
+  {p: x = y} (q: rew [P] p in u = v)
+  {p': y = z} (q': rew [P] p' in v = w):
+  rew [P] eq_trans p p' in u = w.
+Proof.
+  now destruct q', p', q, p.
+Defined.
+
+Infix "⊙" := sigT_trans_eq (at level 65, left associativity).
+
+Notation "q ⊙[ P ] q'" := (@sigT_trans_eq _ P _ _ _ _ _ _ _ q _ q')
+  (at level 65, left associativity, only parsing).
+
+Lemma sigT_trans_eq_refl {A: Type} {P: A -> Type} {x: A} {u v w: P x}
+  (q: u = v) (q': v = w):
+  sigT_trans_eq (p := eq_refl) q (p' := eq_refl) q' = eq_trans q q'.
+Proof.
+  now destruct q', q.
+Defined.
+
+Lemma eq_trans_eq_existT_curried {A: Type} {P: A -> Type}
+  {x y z: A} {u: P x} {v: P y} {w: P z}
+  (p: x = y) (q: rew [P] p in u = v)
+  (p': y = z) (q': rew [P] p' in v = w):
+  eq_trans (= p; q) (= p'; q') =
+  (= eq_trans p p'; sigT_trans_eq q q').
+Proof.
+  now destruct q', p', q, p.
+Defined.
+
+Lemma sigT_trans_eq_existT_curried_dep {A: Type} {P: A -> Type}
+  {Q: {a: A &T P a} -> Type}
+  {x y z: A}
+  {u: P x} {v: Q (x; u)}
+  {u': P y} {v': Q (y; u')}
+  {u'': P z} {v'': Q (z; u'')}
+  (H: x = y) (Hu: rew [P] H in u = u')
+  (Hv: rew [Q] (=H; Hu) in v = v')
+  (H': y = z) (Hu': rew [P] H' in u' = u'')
+  (Hv': rew [Q] (=H'; Hu') in v' = v''):
+  eq_existT_curried_dep (H := H) (Hu := Hu) (Hv := Hv)
+    ⊙ eq_existT_curried_dep (H := H') (Hu := Hu') (Hv := Hv') =
+  eq_existT_curried_dep
+    (H := eq_trans H H')
+    (Hu := Hu ⊙ Hu')
+    (Hv := rew [fun p => rew [Q] p in v = v'']
+      eq_trans_eq_existT_curried H Hu H' Hu' in (Hv ⊙ Hv')).
+Proof.
+  now destruct Hv', Hu', H', Hv, Hu, H.
+Defined.
