theories/νSet/SSGpd.v
@@ -1,0 +1,1143 @@
+Set Warnings "-notation-overridden".
+From Bonak Require Import SigT HSet HGpd Notation LeSProp SSGpdLemmas.
+
+Set Primitive Projections.
+Set Printing Projections.
+Set Keyed Unification.
+
+Module SSGpd.
+
+(** The type of lists {frame(n,0);...;frame(n,p-1)} for arbitrary k := n-p
+    (the non-mandatory dependency in k is useful for type inference) *)
+
+Fixpoint mkFrameTypes p k: Type :=
+  match p with
+  | 0 => unit
+  | S p => { frames: mkFrameTypes p k.+1 &T HGpd }
+  end.
+
+(** The type of lists {painting(n,0);...;painting(n,p-1)} for n := k+p *)
+
+Fixpoint mkPaintingTypes p k: mkFrameTypes p k -> Type :=
+  match p with
+  | 0 => fun _ => unit
+  | S p => fun frames =>
+    { paintings: mkPaintingTypes p k.+1 frames.1 &T frames.2 -> HGpd }
+  end.
+
+(** A helper type so as to mutually build the types of restrFrames and
+    the body of frames using a single fixpoint *)
+
+Class RestrFrameTypeBlock p k := {
+  RestrFrameTypesDef: Type;
+  FrameDef: RestrFrameTypesDef -> mkFrameTypes p.+1 k;
+}.
+
+(**
+For n and p<=n be given, and assuming {frame(n,0);...;frame(n,p)} and
+{painting(n,0);...;painting(n,p)}, we build the list of pairs:
+- of the types RestrFrameTypes(n,p) of the list
+  {restrFrame(n,0);...;restrFrame(n,p-1)}
+  (represented as an inhabitant of a sigma-type
+   {R:RestrFrameTypes(n,0) & ... & RestrFrameTypes(n,p-1)})
+- and of the list {frame(n+1,0);...;frame(n+1,p)} in function of effective
+  restrFrames of type RestrFrameTypes(n,p)
+
+That is, we build:
+- p = 0 : { RestrFrameTypes(n,0..0-1) := unit ;
+                  (which denotes the empty list of restrFrameTypes)
+            Frames(n+1,0..0)(restrFrames^n_{0..0-1}) := {unit}
+                  (representing lists by Sigma-types) }
+- p = 1 : { RestrFrameTypes(n,0..0) = {_:unit & restrFrameType(n,0)} ;
+                  (thus denoting the singleton list {restrFrameType(n,0})
+            Frames(n+1,0..1)(restrFrames(n,0..0) :=
+                  {unit;{d:Frame(n,0)&Painting(n,0)(restrFrame(n,0)(d)}} }
+- ...
+- p     : { RestrFrameTypes(n,0..p-1) =
+              {RestrFrameType(n,0) & ... & RestrFrameType(n,p-1)} ;
+            Frames(n+1,0..p)(restrFrames(n,0..p-1)) :=
+              {frame(n+1,0);...;frame(n+1,p)} }
+
+  In practise, it is convenient to work with the difference k := n-p
+  rather than n itself. So, below, k is the difference.
+*)
+
+Generalizable Variables p k frames.
+
+Definition mkRestrFrameType
+  `(prevFrames: mkFrameTypes p.+1 k.+1)
+   (frames: mkFrameTypes p.+1 k) :=
+  forall q (Hq: q <= k), prevFrames.2 -> frames.2.
+
+Definition mkRestrFrameTypesStep `(frames: mkFrameTypes p.+1 k)
+  (prev: RestrFrameTypeBlock p k.+1) :=
+  { R: prev.(RestrFrameTypesDef) &T mkRestrFrameType (prev.(FrameDef) R) frames }.
+
+Definition mkLayer `{frames: mkFrameTypes p.+1 k}
+  {prevFrames: mkFrameTypes p.+1 k.+1}
+  (restrFrame: mkRestrFrameType prevFrames frames)
+  {painting: frames.2 -> HGpd}
+  (d: prevFrames.2) :=
+  painting (restrFrame 0 leR_O d).
+
+Fixpoint mkRestrFrameTypesAndFrames {p k}:
+  forall `(paintings: mkPaintingTypes p k frames), RestrFrameTypeBlock p k :=
+  match p with
+  | 0 => fun frames paintings =>
+    {|
+      RestrFrameTypesDef := unit;
+      FrameDef _ := (tt; gunit): mkFrameTypes 1 k
+    |}
+  | p.+1 => fun frames paintings =>
+    let prev :=
+      mkRestrFrameTypesAndFrames paintings.1 in
+    let frames' := prev.(FrameDef) in
+    {|
+      RestrFrameTypesDef := mkRestrFrameTypesStep frames prev;
+      FrameDef R :=
+        (frames' R.1; { d: (frames' R.1).2 &
+          mkLayer R.2 (painting := paintings.2) d }): mkFrameTypes p.+2 k
+    |}
+  end.
+
+Definition mkRestrFrameTypes `(paintings: mkPaintingTypes p k frames) :=
+  (mkRestrFrameTypesAndFrames paintings).(RestrFrameTypesDef).
+
+Class DepsRestr p k := {
+  _frames: mkFrameTypes p k;
+  _paintings: mkPaintingTypes p k _frames;
+  _restrFrames: mkRestrFrameTypes _paintings;
+}.
+
+Instance toDepsRestr `{paintings: mkPaintingTypes p k frames}
+  (restrFrames: mkRestrFrameTypes paintings) : DepsRestr p k :=
+  {| _restrFrames := restrFrames |}.
+
+#[local]
+Instance proj1DepsRestr `(deps: DepsRestr p.+1 k): DepsRestr p k.+1 :=
+{|
+  _frames := deps.(_frames).1;
+  _paintings := deps.(_paintings).1;
+  _restrFrames := deps.(_restrFrames).1;
+|}.
+
+Declare Scope depsrestr_scope.
+Delimit Scope depsrestr_scope with depsrestr.
+Bind Scope depsrestr_scope with DepsRestr.
+Notation "x .(1)" := (proj1DepsRestr x%_depsrestr)
+  (at level 1, left associativity, format "x .(1)"): depsrestr_scope.
+
+Definition mkFrames `(deps: DepsRestr p k): mkFrameTypes p.+1 k :=
+  (mkRestrFrameTypesAndFrames
+    deps.(_paintings)).(FrameDef) deps.(_restrFrames).
+
+Definition mkFrame `(deps: DepsRestr p k): HGpd := (mkFrames deps).2.
+
+Inductive DepsRestrExtension p: forall k, DepsRestr p k -> Type :=
+| TopRestrDep {deps} (E: mkFrame deps -> HGpd): DepsRestrExtension p 0 deps
+| AddRestrDep {k} deps:
+  DepsRestrExtension p.+1 k deps -> DepsRestrExtension p k.+1 deps.(1).
+
+Arguments TopRestrDep {p deps}.
+Arguments AddRestrDep {p k} deps.
+
+Declare Scope extra_depsrestr_scope.
+Delimit Scope extra_depsrestr_scope with extradepsrestr.
+Bind Scope extra_depsrestr_scope with DepsRestrExtension.
+Notation "( x ; y )" := (AddRestrDep x y)
+  (at level 0, format "( x ; y )"): extra_depsrestr_scope.
+
+(* Example: if p := 0, extraDeps := ({},E) mkPainting:= {E} *)
+
+Generalizable Variables deps.
+
+Fixpoint mkPainting `(extraDeps: DepsRestrExtension p k deps):
+  mkFrame deps -> HGpd :=
+  match extraDeps with
+  | TopRestrDep E => fun d => E d
+  | AddRestrDep deps extraDeps => fun (d: mkFrame deps.(1)) =>
+      {l: mkLayer deps.(_restrFrames).2 d & mkPainting extraDeps (d; l)}
+  end.
+
+Fixpoint mkPaintingsPrefix {p k}:
+  forall `(extraDeps: DepsRestrExtension p k deps),
+    mkPaintingTypes p k.+1 (mkFrames deps).1 :=
+  match p with
+  | 0 => fun _ _ => tt
+  | S p => fun deps extraDeps =>
+      (mkPaintingsPrefix (deps; extraDeps)%extradepsrestr;
+       mkPainting (deps; extraDeps)%extradepsrestr)
+  end.
+
+Definition mkPaintings {p k}: forall `(extraDeps: DepsRestrExtension p k deps),
+  mkPaintingTypes p.+1 k (mkFrames deps) :=
+  fun deps extraDeps => (mkPaintingsPrefix extraDeps; mkPainting extraDeps).
+
+Definition mkRestrPaintingType
+  `(extraDeps: DepsRestrExtension p.+1 k deps) :=
+  forall q (Hq: q <= k) (d: mkFrame deps.(1)),
+  (mkPaintings (deps; extraDeps)).2 d ->
+  deps.(_paintings).2 (deps.(_restrFrames).2 q Hq d).
+
+Fixpoint mkRestrPaintingTypes {p}:
+  forall `(extraDeps: DepsRestrExtension p k deps), Type :=
+  match p with
+  | 0 => fun _ _ _ => unit
+  | S p =>
+    fun k deps extraDeps =>
+    { _: mkRestrPaintingTypes (deps; extraDeps) &T
+      mkRestrPaintingType extraDeps }
+  end.
+
+(** A helper type so as to mutually build the types of cohFrames and
+    the body of restrFrames using a single fixpoint *)
+
+Class CohFrameTypeBlock `{extraDeps: DepsRestrExtension p k deps} := {
+  CohFrameTypesDef: Type;
+  RestrFramesDef: CohFrameTypesDef -> mkRestrFrameTypes (mkPaintings extraDeps)
+}.
+
+(** Auxiliary definitions to mutually build cohFrameTypes and restrFrames *)
+
+Definition mkCohFrameType `{extraDeps: DepsRestrExtension p.+1 k deps}
+  (prevRestrFrames: mkRestrFrameTypes (mkPaintings (deps; extraDeps))): Type :=
+  forall q (Hq: q <= k) r (Hr: r <= q)
+    (d: mkFrame (toDepsRestr prevRestrFrames).(1)),
+  deps.(_restrFrames).2 q Hq (prevRestrFrames.2 r (Hr ↕ (↑ Hq)) d) =
+  deps.(_restrFrames).2 r (Hr ↕ Hq) (prevRestrFrames.2 q.+1 (⇑ Hq) d).
+
+Definition mkCohFrameTypesStep `{extraDeps: DepsRestrExtension p.+1 k deps}
+  (prev: CohFrameTypeBlock (extraDeps := (deps; extraDeps))): Type :=
+  { Q: prev.(CohFrameTypesDef) &T mkCohFrameType (prev.(RestrFramesDef) Q) }.
+
+Definition mkRestrLayer `{extraDeps: DepsRestrExtension p.+1 k deps}
+  {prevRestrFrames: mkRestrFrameTypes (mkPaintings (deps;extraDeps))}
+  (restrPainting: mkRestrPaintingType extraDeps)
+  (cohFrame: mkCohFrameType prevRestrFrames)
+  q (Hq: q <= k)
+  (d: mkFrame (toDepsRestr prevRestrFrames).(1))
+  (l: mkLayer prevRestrFrames.2 d):
+  mkLayer deps.(_restrFrames).2 (prevRestrFrames.2 q.+1 (⇑ Hq) d) :=
+    rew [deps.(_paintings).2] cohFrame q Hq 0 leR_O d in
+    restrPainting q Hq _ l.
+
+(** Under previous assumptions, and, additionally:
+    - {restrPainting(n,0);...;restrPainting(n,p-1)}
+    we mutually build the pair of:
+    - the list of types for {cohFrame(n,0);...;cohFrame(n,p-1)}
+    - definitions of {restrFrame(n+1,0);...;restrFrame(n+1,p)} *)
+
+Fixpoint mkCohFrameTypesAndRestrFrames {p k}:
+  forall `{extraDeps: DepsRestrExtension p k deps}
+  (restrPaintings: mkRestrPaintingTypes extraDeps), CohFrameTypeBlock :=
+  match p with
+  | 0 =>
+    fun deps extraDeps restrPaintings =>
+    {|
+      CohFrameTypesDef := unit;
+      RestrFramesDef _ := (tt; fun _ _ _ => tt)
+    |}
+  | S p =>
+    fun deps extraDeps restrPaintings =>
+    let prev := mkCohFrameTypesAndRestrFrames restrPaintings.1 in
+    let restrFrames := prev.(RestrFramesDef) in
+    {|
+      CohFrameTypesDef := mkCohFrameTypesStep prev;
+      RestrFramesDef Q :=
+      let restrFrame q (Hq: q <= k)
+        (d: mkFrame (toDepsRestr (restrFrames Q.1))) :=
+          ((restrFrames Q.1).2 q.+1 (⇑ Hq) d.1;
+           mkRestrLayer restrPaintings.2 Q.2 q _ d.1 d.2)
+      in (restrFrames Q.1; restrFrame)
+    |}
+  end.
+
+(* Example: if p := 0, extraDeps := ({},E)
+   mkCohFrameTypes := {} *)
+
+Definition mkCohFrameTypes `{extraDeps: DepsRestrExtension p k deps}
+  (restrPaintings: mkRestrPaintingTypes extraDeps) :=
+  (mkCohFrameTypesAndRestrFrames restrPaintings).(CohFrameTypesDef).
+
+Class DepsCohs p k := {
+  _deps: DepsRestr p k;
+  _extraDeps: DepsRestrExtension p k _deps;
+  _restrPaintings: mkRestrPaintingTypes _extraDeps;
+  _cohs: mkCohFrameTypes _restrPaintings;
+}.
+
+#[local]
+Instance toDepsCohs `{extraDeps: DepsRestrExtension p k deps}
+  {restrPaintings: mkRestrPaintingTypes extraDeps}
+  (cohs: mkCohFrameTypes restrPaintings): DepsCohs p k :=
+  {| _cohs := cohs |}.
+
+#[local]
+Instance proj1DepsCohs `(depsCohs: DepsCohs p.+1 k): DepsCohs p k.+1 :=
+{|
+  _deps := depsCohs.(_deps).(1);
+  _extraDeps := (depsCohs.(_deps); depsCohs.(_extraDeps));
+  _restrPaintings := depsCohs.(_restrPaintings).1;
+  _cohs := depsCohs.(_cohs).1;
+|}.
+
+Declare Scope depscohs_scope.
+Delimit Scope depscohs_scope with depscohs.
+Bind Scope depscohs_scope with DepsCohs.
+Notation "x .(1)" := (proj1DepsCohs x%depscohs)
+  (at level 1, left associativity, format "x .(1)"): depscohs_scope.
+
+(** The restrFrame(n+1,0..p) component of the fixpoint *)
+
+Definition mkRestrFrames `{depsCohs: DepsCohs p k} :=
+  (mkCohFrameTypesAndRestrFrames depsCohs.(_restrPaintings)).(RestrFramesDef)
+    depsCohs.(_cohs).
+
+(** For n=p+k, we combine mkFrames (that is frames(n+1,p)),
+    mkPaintings (that is paintings(n+1,p)) and restrFrames
+    (that is restrFrames(n+1,p)) to build "dependencies" at the next
+    level, that is a deps(n+1,p).
+    That is, from:
+     - {frame(n,0);...;frame(n,p-1)}
+     - {painting(n,0);...;painting(n,p-1)}
+     - {restrFrame(n,0);...;restrFrame(n,p-1)} for p<=n+1
+     (forming a "deps"), and
+     - {frame(n,p);...;frame(n,n)}
+     - {painting(n,p);...;painting(n,n)}
+     - {restrFrame(n,p);...;restrFrame(n,n)}
+     - E:frame(n+1,n+1) -> HGpd
+     (forming an "extraDeps")
+     we form:
+     - {frame(n+1,0);...;frame(n+1,p)} (built by mkFrames)
+     - {painting(n+1,0);...;painting(p+n,p)} (built by mkPaintings)
+     - {restrFrame(n+1,0);...;restrFrame(n+1,p)} (built by mkRestrFrames)
+
+   Example: if p := 0, extraDeps := ({},E), restrPaintings := {}, cohs := {}
+   then mkDepsRestr := {frames'':={unit};
+                        paintings'':={E};
+                        restrFrames':={λq().()}}
+   (where restrFrames' is presented as a dependent pair, i.e. ((),λq().()) *)
+
+Definition mkDepsRestr `{depsCohs: DepsCohs p k} :=
+  toDepsRestr mkRestrFrames.
+
+(** Deducing restrFrame(n+1,p) *)
+
+(** Note that we use mkRestrFrames(n+1,p) both to build frame(n+2,p) and
+    restrFrame(n+1,p) : frame(n+2,p) -> frame(n+1,p), according to the
+    circularity between Frames and RestrFrameTypes.
+    But now, thanks to restrPaintings and cohFrames, we have an effective
+    definition of RestrFrame(n+1,p) and the circular dependency of
+    frame(n+2,p) with an inhabitant RestrFrame(n+1,p) of RestrFrameType(n+1,p)
+    is gone.
+ *)
+
+Definition mkRestrFrame `{depsCohs: DepsCohs p k}:
+  forall q (Hq: q <= k),
+  mkFrame mkDepsRestr.(1) -> mkFrame depsCohs.(_deps) :=
+  mkRestrFrames.2.
+
+Inductive DepsCohsExtension p: forall k (depsCohs: DepsCohs p k), Type :=
+| TopCohDep `{depsCohs: DepsCohs p 0}
+  (E: mkFrame mkDepsRestr -> HGpd):
+  DepsCohsExtension p 0 depsCohs
+| AddCohDep {k} (depsCohs: DepsCohs p.+1 k):
+  DepsCohsExtension p.+1 k depsCohs -> DepsCohsExtension p k.+1 depsCohs.(1).
+
+Arguments TopCohDep {p depsCohs}.
+Arguments AddCohDep {p k}.
+
+Declare Scope extra_depscohs_scope.
+Delimit Scope extra_depscohs_scope with extradepscohs.
+Bind Scope extra_depscohs_scope with DepsCohsExtension.
+Notation "( x ; y )" := (AddCohDep x y)
+  (at level 0, format "( x ; y )"): extra_depscohs_scope.
+
+Generalizable Variables depsCohs.
+
+Fixpoint mkExtraDeps `(extraDepsCohs: DepsCohsExtension p k depsCohs):
+  DepsRestrExtension p.+1 k mkDepsRestr.
+Proof.
+  destruct extraDepsCohs.
+  - now constructor.
+  - apply (AddRestrDep mkDepsRestr
+    (mkExtraDeps p.+1 k depsCohs extraDepsCohs)).
+Defined.
+
+Fixpoint mkRestrPainting `(extraDepsCohs: DepsCohsExtension p k depsCohs)
+  q {struct q}:
+  forall (Hq: q <= k) (d: mkFrame mkDepsRestr.(1)),
+    (mkPaintings (mkDepsRestr; mkExtraDeps extraDepsCohs)).2 d ->
+    mkDepsRestr.(_paintings).2 (mkDepsRestr.(_restrFrames).2 q Hq d).
+Proof.
+  destruct q as [|q]; intros Hq d [l c].
+  - exact l.
+  - destruct extraDepsCohs as [|k0 depsCohs0 extraDepsCohs0].
+    + now destruct (leR_O_contra Hq).
+    + unshelve eapply existT.
+      * exact (mkRestrLayer depsCohs0.(_restrPaintings).2 depsCohs0.(_cohs).2
+          q (⇓ Hq) d l).
+      * exact (mkRestrPainting _ _ _ extraDepsCohs0 q (⇓ Hq) (d; l) c).
+Defined.
+
+Fixpoint mkRestrPaintingsPrefix {p k}:
+  forall `(extraDepsCohs: DepsCohsExtension p k depsCohs),
+  mkRestrPaintingTypes
+    (mkDepsRestr; mkExtraDeps extraDepsCohs)%extradepsrestr :=
+  match p with
+  | 0 => fun _ _ => tt
+  | S p =>
+    fun depsCohs extraDepsCohs =>
+      (mkRestrPaintingsPrefix (depsCohs; extraDepsCohs)%extradepscohs;
+       mkRestrPainting (depsCohs; extraDepsCohs)%extradepscohs)
+  end.
+
+Definition mkRestrPaintings {p k}:
+  forall `(extraDepsCohs: DepsCohsExtension p k depsCohs),
+  mkRestrPaintingTypes (mkExtraDeps extraDepsCohs) :=
+  fun depsCohs extraDepsCohs => (mkRestrPaintingsPrefix extraDepsCohs; mkRestrPainting extraDepsCohs).
+
+(** The groupoid-level replacement for the old [mkCoh2Frame] UIP proof:
+    this is now explicit 2-dimensional frame coherence data. *)
+
+Definition mkCoh2FrameType
+  `(extraDepsCohs: DepsCohsExtension p.+1 k depsCohs)
+  (prevCohFrames: mkCohFrameTypes
+    (mkRestrPaintings (depsCohs; extraDepsCohs))): Type :=
+  forall q (Hq: q <= k) r (Hr: r <= q) s (Hs: s <= r)
+    (d: mkFrame (mkDepsRestr (depsCohs := toDepsCohs prevCohFrames.1)).(1)),
+  f_equal
+    (fun x => depsCohs.(_deps).(_restrFrames).2 q _ x)
+    (prevCohFrames.2 r (Hr ↕ ↑ Hq) s Hs d)
+  • (depsCohs.(_cohs).2 q Hq s (Hs ↕ Hr)
+      (mkRestrFrame r.+1 (⇑ (Hr ↕ ↑ Hq)) d)
+  • f_equal
+      (fun x => depsCohs.(_deps).(_restrFrames).2 s (Hs ↕ (Hr ↕ Hq)) x)
+      (prevCohFrames.2 q.+1 (⇑ Hq) r.+1 (⇑ Hr) d)) =
+  depsCohs.(_cohs).2 q Hq r Hr
+    (mkRestrFrame s (↑ (↑ (Hs ↕ (Hr ↕ Hq)))) d)
+  • (f_equal
+      (fun x => depsCohs.(_deps).(_restrFrames).2 r _ x)
+      (prevCohFrames.2 q.+1 (⇑ Hq) s (↑ (Hs ↕ Hr)) d)
+  • depsCohs.(_cohs).2 r (Hr ↕ Hq) s Hs
+      (mkRestrFrame q.+2 (⇑ (⇑ Hq)) d)).
+
+Definition mkCohPaintingType
+  `(extraDepsCohs: DepsCohsExtension p.+1 k depsCohs) :=
+  forall q (Hq: q <= k) r (Hr: r <= q)
+    (d: mkFrame mkDepsRestr.(1))
+    (c: (mkPaintings (mkDepsRestr;
+      mkExtraDeps (depsCohs; extraDepsCohs))).2 d),
+  rew [depsCohs.(_deps).(_paintings).2] depsCohs.(_cohs).2 q Hq r Hr d in
+  depsCohs.(_restrPaintings).2 q Hq _
+    ((mkRestrPaintings (depsCohs; extraDepsCohs)).2 r _ d c) =
+  depsCohs.(_restrPaintings).2 r (Hr ↕ Hq) _
+    ((mkRestrPaintings (depsCohs; extraDepsCohs)).2 q.+1 _ d c).
+
+Fixpoint mkCohPaintingTypes {p}:
+  forall `(extraDepsCohs: DepsCohsExtension p k depsCohs), Type :=
+  match p with
+  | 0 => fun _ _ _ => unit
+  | S p =>
+    fun k depsCohs extraDepsCohs =>
+    { R: mkCohPaintingTypes (depsCohs; extraDepsCohs) &T
+         mkCohPaintingType extraDepsCohs }
+  end.
+
+Definition mkCohLayerType `{extraDepsCohs: DepsCohsExtension p.+1 k depsCohs}
+  {prevCohFrames: mkCohFrameTypes
+    (extraDeps := (mkDepsRestr; mkExtraDeps extraDepsCohs))
+    (mkRestrPaintings extraDepsCohs).1}
+  q (Hq: q <= k) r (Hr: r <= q)
+  (d: mkFrame (mkDepsRestr (depsCohs := toDepsCohs prevCohFrames.1)).(1))
+  (l: mkLayer mkRestrFrame d): Type :=
+  rew [mkLayer _] prevCohFrames.2 q.+1 (⇑ Hq) r.+1 (⇑ Hr) d in
+  mkRestrLayer depsCohs.(_restrPaintings).2 depsCohs.(_cohs).2 q Hq _
+    (mkRestrLayer (mkRestrPaintings extraDepsCohs).1.2 prevCohFrames.2 r (Hr ↕ ↑ Hq) d l) =
+  mkRestrLayer depsCohs.(_restrPaintings).2 depsCohs.(_cohs).2 r (Hr ↕ Hq) _
+    (mkRestrLayer (mkRestrPaintings extraDepsCohs).1.2 prevCohFrames.2 q.+1 (⇑ Hq) d l).
+
+Definition mkCohLayer `{extraDepsCohs: DepsCohsExtension p.+1 k depsCohs}
+  {prevCohFrames: mkCohFrameTypes
+    (extraDeps := (mkDepsRestr; mkExtraDeps extraDepsCohs))
+    (mkRestrPaintings extraDepsCohs).1}
+  (cohPainting: mkCohPaintingType extraDepsCohs)
+  (coh2Frame: mkCoh2FrameType extraDepsCohs prevCohFrames)
+  q (Hq: q <= k) r (Hr: r <= q)
+  (d: mkFrame (mkDepsRestr (depsCohs := toDepsCohs prevCohFrames.1)).(1))
+  (l: mkLayer mkRestrFrame d):
+  mkCohLayerType q Hq r Hr d l.
+Proof.
+  unfold mkCohLayerType, mkRestrLayer, mkLayer.
+  eapply rew_cohLayer with
+    (P := fun x => depsCohs.(_deps).(_paintings).2 x)
+    (rf0 := fun x => depsCohs.(_deps).(_restrFrames).2 0 leR_O x)
+    (F := depsCohs.(_restrPaintings).2 q Hq)
+    (G := depsCohs.(_restrPaintings).2 r (Hr ↕ Hq)).
+  - now exact (cohPainting q Hq r Hr
+      (((mkCohFrameTypesAndRestrFrames (mkRestrPaintings extraDepsCohs).1.1)
+        .(RestrFramesDef) prevCohFrames.1).2 0 leR_O d) l).
+  - now apply (coh2Frame q Hq r Hr 0 leR_O d).
+Defined.
+
+Class Coh2FrameTypeBlock `{extraDepsCohs: DepsCohsExtension p k depsCohs} := {
+  Coh2FrameTypesDef: Type;
+  CohFramesDef: Coh2FrameTypesDef -> mkCohFrameTypes (mkRestrPaintings extraDepsCohs);
+}.
+
+Definition mkCoh2FrameTypesStep
+  `{extraDepsCohs: DepsCohsExtension p.+1 k depsCohs}
+  (cohPaintings: mkCohPaintingTypes extraDepsCohs)
+  (prev: Coh2FrameTypeBlock
+    (extraDepsCohs := (depsCohs; extraDepsCohs)%extradepscohs)): Type :=
+  { R: prev.(Coh2FrameTypesDef) &T
+    mkCoh2FrameType extraDepsCohs (prev.(CohFramesDef) R) }.
+
+Fixpoint mkCoh2FrameTypesAndCohFrames {p k}:
+  forall `{extraDepsCohs: DepsCohsExtension p k depsCohs}
+  (cohPaintings: mkCohPaintingTypes extraDepsCohs),
+  Coh2FrameTypeBlock (extraDepsCohs := extraDepsCohs).
+Proof.
+  destruct p.
+  - intros depsCohs extraDepsCohs cohPaintings.
+    unshelve econstructor.
+    + now exact unit.
+    + intros _. unshelve esplit. now exact tt. now intros.
+  - intros depsCohs extraDepsCohs cohPaintings.
+    set (prev := mkCoh2FrameTypesAndCohFrames p k.+1
+      depsCohs.(1)%depscohs
+      (depsCohs; extraDepsCohs)%extradepscohs cohPaintings.1).
+    unshelve econstructor.
+    + now exact (mkCoh2FrameTypesStep cohPaintings prev).
+    + intros Q.
+      set (h := prev.(CohFramesDef) Q.1).
+      unshelve esplit. now exact h.
+      intros q Hq r Hr d.
+      unshelve eapply eq_existT_curried.
+      * now exact (h.2 q.+1 (⇑ Hq) r.+1 (⇑ Hr) d.1).
+      * now exact (mkCohLayer cohPaintings.2 Q.2 q Hq r Hr d.1 d.2).
+Defined.
+
+Definition mkCoh2FrameTypes `{extraDepsCohs: DepsCohsExtension p k depsCohs}
+  (cohPaintings: mkCohPaintingTypes extraDepsCohs) :=
+  (mkCoh2FrameTypesAndCohFrames cohPaintings).(Coh2FrameTypesDef).
+
+Definition mkCohFrames `{extraDepsCohs: DepsCohsExtension p k depsCohs}
+  (cohPaintings: mkCohPaintingTypes extraDepsCohs)
+  (coh2Frames: mkCoh2FrameTypes cohPaintings):
+  mkCohFrameTypes (mkRestrPaintings extraDepsCohs) :=
+  (mkCoh2FrameTypesAndCohFrames cohPaintings).(CohFramesDef) coh2Frames.
+
+Definition mkCohFrame `{extraDepsCohs: DepsCohsExtension p k depsCohs}
+  (cohPaintings: mkCohPaintingTypes extraDepsCohs)
+  (coh2Frames: mkCoh2FrameTypes cohPaintings):
+  mkCohFrameType (mkRestrFrames (depsCohs :=
+    toDepsCohs (mkCohFrames cohPaintings coh2Frames).1)) :=
+  (mkCohFrames cohPaintings coh2Frames).2.
+
+Class DepsCohs2 p k := {
+  _depsCohs: DepsCohs p k;
+  _extraDepsCohs: DepsCohsExtension p k _depsCohs;
+  _cohPaintings: mkCohPaintingTypes _extraDepsCohs;
+  _coh2Frames: mkCoh2FrameTypes _cohPaintings;
+}.
+
+#[local]
+Instance toDepsCohs2 `{extraDepsCohs: DepsCohsExtension p k depsCohs}
+  {cohPaintings: mkCohPaintingTypes extraDepsCohs}
+  (coh2Frames: mkCoh2FrameTypes cohPaintings): DepsCohs2 p k :=
+  {| _coh2Frames := coh2Frames |}.
+
+#[local]
+Instance proj1DepsCohs2 `(depsCohs2: DepsCohs2 p.+1 k): DepsCohs2 p k.+1 :=
+{|
+  _depsCohs := depsCohs2.(_depsCohs).(1);
+  _extraDepsCohs := (depsCohs2.(_depsCohs); depsCohs2.(_extraDepsCohs));
+  _cohPaintings := depsCohs2.(_cohPaintings).1;
+  _coh2Frames := depsCohs2.(_coh2Frames).1;
+|}.
+
+Declare Scope depscohs2_scope.
+Delimit Scope depscohs2_scope with depscohs2.
+Bind Scope depscohs2_scope with DepsCohs2.
+Notation "x .(1)" := (proj1DepsCohs2 x%depscohs2)
+  (at level 1, left associativity, format "x .(1)"): depscohs2_scope.
+
+#[local]
+Instance mkDepsCohs `(depsCohs2: DepsCohs2 p k): DepsCohs p.+1 k :=
+{|
+  _deps := mkDepsRestr;
+  _extraDeps := mkExtraDeps depsCohs2.(_extraDepsCohs);
+  _restrPaintings := mkRestrPaintings depsCohs2.(_extraDepsCohs);
+  _cohs := mkCohFrames depsCohs2.(_cohPaintings) depsCohs2.(_coh2Frames);
+|}.
+
+Inductive DepsCohs2Extension p: forall k (depsCohs2: DepsCohs2 p k), Type :=
+| TopCoh2Dep `{depsCohs2: DepsCohs2 p 0}
+  (E: mkFrame (mkDepsRestr (depsCohs := mkDepsCohs depsCohs2)) -> HGpd):
+  DepsCohs2Extension p 0 depsCohs2
+| AddCoh2Dep {k} (depsCohs2: DepsCohs2 p.+1 k):
+  DepsCohs2Extension p.+1 k depsCohs2 ->
+  DepsCohs2Extension p k.+1 depsCohs2.(1).
+
+Arguments TopCoh2Dep {p depsCohs2}.
+Arguments AddCoh2Dep {p k}.
+
+Declare Scope extra_depscohs2_scope.
+Delimit Scope extra_depscohs2_scope with extradepscohs2.
+Bind Scope extra_depscohs2_scope with DepsCohs2Extension.
+Notation "( x ; y )" := (AddCoh2Dep x y)
+  (at level 0, format "( x ; y )"): extra_depscohs2_scope.
+
+Fixpoint mkExtraCohs `{depsCohs2: DepsCohs2 p k}
+  (extraDepsCohs2: DepsCohs2Extension p k depsCohs2):
+  DepsCohsExtension p.+1 k (mkDepsCohs depsCohs2).
+Proof.
+  destruct extraDepsCohs2.
+  - now constructor.
+  - apply (AddCohDep (mkDepsCohs depsCohs2)).
+    now exact (mkExtraCohs p.+1 k depsCohs2 extraDepsCohs2).
+Defined.
+
+Definition mkCohPainting `{depsCohs2: DepsCohs2 p k}
+  (extraDepsCohs2: DepsCohs2Extension p k depsCohs2):
+  mkCohPaintingType (mkExtraCohs extraDepsCohs2).
+Proof.
+  intros q Hq r.
+  generalize dependent q.
+  generalize dependent k.
+  generalize dependent p.
+  induction r as [|r mkCohPainting].
+  - now intros.
+  - intros p k depsCohs2 extraDepsCohs2 q Hq Hr d c.
+    destruct q; [now contradict Hq |].
+    destruct extraDepsCohs2; [now contradict Hq |].
+    destruct c as [l c].
+    unshelve eapply (eq_existT_curried_dep
+      (Q := mkPainting depsCohs2.(_depsCohs).(_extraDeps))).
+    + now exact (mkCohLayer depsCohs2.(_cohPaintings).2 depsCohs2.(_coh2Frames).2
+        q (⇓ Hq) r (⇓ Hr) d l).
+    + now exact (mkCohPainting p.+1 k depsCohs2 extraDepsCohs2
+        q (⇓ Hq) (⇓ Hr) (d; l) c).
+Defined.
+
+Fixpoint mkCohPaintingsPrefix `{depsCohs2: DepsCohs2 p k}
+  (extraDepsCohs2: DepsCohs2Extension p k depsCohs2) {struct p}:
+  @mkCohPaintingTypes p k.+1 (mkDepsCohs depsCohs2).(1)
+    (mkDepsCohs depsCohs2; mkExtraCohs extraDepsCohs2)%extradepscohs.
+Proof.
+  destruct p.
+  - now exact tt.
+  - unshelve esplit.
+    + now exact (mkCohPaintingsPrefix p k.+1 depsCohs2.(1)%depscohs2
+        (depsCohs2; extraDepsCohs2)%extradepscohs2).
+    + now exact (mkCohPainting (depsCohs2; extraDepsCohs2)%extradepscohs2).
+Defined.
+
+Definition mkCohPaintings `{depsCohs2: DepsCohs2 p k}
+  (extraDepsCohs2: DepsCohs2Extension p k depsCohs2):
+  mkCohPaintingTypes (mkExtraCohs extraDepsCohs2) :=
+  (mkCohPaintingsPrefix extraDepsCohs2; mkCohPainting extraDepsCohs2).
+
+Definition mkCoh2PaintingSourcePainting {p k}
+  (depsCohs2: DepsCohs2 p.+1 k)
+  (extraDepsCohs2: DepsCohs2Extension p.+1 k depsCohs2)
+  (d: mkFrame ((mkDepsRestr (depsCohs := (mkDepsCohs depsCohs2).(1).(1)))).(1)): HGpd :=
+  (mkPaintings ((mkDepsRestr (depsCohs := mkDepsCohs depsCohs2)).(1).(1);
+    mkExtraDeps ((mkDepsCohs depsCohs2).(1); (mkDepsCohs depsCohs2;
+      mkExtraCohs extraDepsCohs2)))).2 d.
+
+Definition mkCoh2PaintingFrameEndpointType {p k}
+  (depsCohs2: DepsCohs2 p.+1 k)
+  q (Hq: q <= k) r (Hr: r <= q) s (Hs: s <= r)
+  (d: mkFrame (mkDepsRestr (depsCohs := (mkDepsCohs depsCohs2).(1).(1))).(1)): Type :=
+  depsCohs2.(_depsCohs).(_deps).(_restrFrames).2 q Hq
+    (mkRestrFrame (depsCohs := depsCohs2.(_depsCohs).(1)) r (Hr ↕ ↑ Hq)
+      (mkRestrFrame s (Hs ↕ ↑ (Hr ↕ ↑ Hq)) d)) =
+  depsCohs2.(_depsCohs).(_deps).(_restrFrames).2 s (Hs ↕ (Hr ↕ Hq))
+    (mkRestrFrame (depsCohs := depsCohs2.(_depsCohs).(1)) r.+1 (⇑ Hr ↕ ⇑ Hq)
+      (mkRestrFrame q.+2 (⇑ (⇑ Hq)) d)).
+
+Definition mkCoh2PaintingEndpointType {p k}
+  (depsCohs2: DepsCohs2 p.+1 k)
+  (extraDepsCohs2: DepsCohs2Extension p.+1 k depsCohs2)
+  q (Hq: q <= k) r (Hr: r <= q) s (Hs: s <= r)
+  (d: mkFrame (mkDepsRestr (depsCohs := (mkDepsCohs depsCohs2).(1).(1))).(1))
+  (c: mkCoh2PaintingSourcePainting depsCohs2 extraDepsCohs2 d)
+  (coh2FrameEndpoint: mkCoh2PaintingFrameEndpointType
+    depsCohs2 q Hq r Hr s Hs d): Type :=
+  let restrPainting1 := mkRestrPainting
+    (depsCohs2.(_depsCohs); depsCohs2.(_extraDepsCohs)) in
+  let restrPainting2 := mkRestrPainting ((mkDepsCohs depsCohs2).(1);
+    (mkDepsCohs depsCohs2; mkExtraCohs extraDepsCohs2)) in
+  rew [depsCohs2.(_depsCohs).(_deps).(_paintings).2] coh2FrameEndpoint in
+  depsCohs2.(_depsCohs).(_restrPaintings).2 q Hq _
+    (restrPainting1 r (Hr ↕ ↑ Hq) _
+      (restrPainting2 s (Hs ↕ ↑ (Hr ↕ ↑ Hq)) d c)) =
+  depsCohs2.(_depsCohs).(_restrPaintings).2 s (Hs ↕ (Hr ↕ Hq)) _
+    (restrPainting1 r.+1 (⇑ Hr ↕ ⇑ Hq) _
+      (restrPainting2 q.+2 (⇑ (⇑ Hq)) d c)).
+
+(** The instance body is a named definition so that goals stay one line:
+    tactics like [destruct] re-typecheck their motive, which is
+    prohibitive over the unfolded body (observed: ~28s for
+    [destruct c] in [mkCoh2Painting] on the raw body, negligible once
+    folded). *)
+Definition mkCoh2PaintingInstanceType {p k}
+  (depsCohs2: DepsCohs2 p.+1 k)
+  (extraDepsCohs2: DepsCohs2Extension p.+1 k depsCohs2)
+  q (Hq: q <= k) r (Hr: r <= q) s (Hs: s <= r)
+  (d: mkFrame (mkDepsRestr (depsCohs := (mkDepsCohs depsCohs2).(1).(1))).(1))
+  (c: mkCoh2PaintingSourcePainting depsCohs2 extraDepsCohs2 d): Type :=
+  let depsCohs := depsCohs2.(_depsCohs) in
+  let restrPainting2 := mkRestrPainting ((mkDepsCohs depsCohs2).(1);
+    (mkDepsCohs depsCohs2; mkExtraCohs extraDepsCohs2)) in
+  rew [mkCoh2PaintingEndpointType depsCohs2 extraDepsCohs2 q Hq r Hr s Hs d c]
+    depsCohs2.(_coh2Frames).2 q Hq r Hr s Hs d in
+  (sigT_map_eq (Q := fun x => GDom (depsCohs.(_deps).(_paintings).2 x))
+    (depsCohs.(_restrPaintings).2 q Hq)
+    (mkCohPainting (depsCohs2; extraDepsCohs2) r (Hr ↕ ↑ Hq) s Hs d c)
+  ⊙ (depsCohs2.(_cohPaintings).2 q Hq s (Hs ↕ Hr)
+      (mkRestrFrame r.+1 (⇑ (Hr ↕ ↑ Hq)) d)
+      (restrPainting2 r.+1 (⇑ (Hr ↕ ↑ Hq)) d c)
+  ⊙[fun x => GDom (depsCohs.(_deps).(_paintings).2 x)]
+    sigT_map_eq (Q := fun x => GDom (depsCohs.(_deps).(_paintings).2 x))
+      (depsCohs.(_restrPaintings).2 s (Hs ↕ (Hr ↕ Hq)))
+      (mkCohPainting (depsCohs2; extraDepsCohs2) q.+1 (⇑ Hq) r.+1 (⇑ Hr) d c))) =
+  depsCohs2.(_cohPaintings).2 q Hq r Hr
+    (mkRestrFrame s (↑ (↑ (Hs ↕ (Hr ↕ Hq)))) d)
+    (restrPainting2 s (↑ (↑ (Hs ↕ (Hr ↕ Hq)))) d c)
+  ⊙[fun x => GDom (depsCohs.(_deps).(_paintings).2 x)]
+    (sigT_map_eq (Q := fun x => GDom (depsCohs.(_deps).(_paintings).2 x))
+      (depsCohs.(_restrPaintings).2 r (Hr ↕ Hq))
+      (mkCohPainting (depsCohs2; extraDepsCohs2) q.+1 (⇑ Hq) s (↑ (Hs ↕ Hr)) d c)
+  ⊙ depsCohs2.(_cohPaintings).2 r (Hr ↕ Hq) s Hs
+      (mkRestrFrame q.+2 (⇑ (⇑ Hq)) d)
+      (restrPainting2 q.+2 (⇑ (⇑ Hq)) d c)).
+
+Definition mkCoh2PaintingType {p k}
+  (depsCohs2: DepsCohs2 p.+1 k)
+  (extraDepsCohs2: DepsCohs2Extension p.+1 k depsCohs2): Type :=
+  forall
+  q (Hq: q <= k) r (Hr: r <= q) s (Hs: s <= r)
+  (d: mkFrame (mkDepsRestr (depsCohs := (mkDepsCohs depsCohs2).(1).(1))).(1))
+  (c: mkCoh2PaintingSourcePainting depsCohs2 extraDepsCohs2 d),
+  mkCoh2PaintingInstanceType depsCohs2 extraDepsCohs2 q Hq r Hr s Hs d c.
+
+Fixpoint mkCoh2PaintingTypes {p}:
+  forall `{extraDepsCohs2: DepsCohs2Extension p k depsCohs2}, Type :=
+  match p with
+  | 0 => fun _ _ _ => unit
+  | S p =>
+    fun k depsCohs2 extraDepsCohs2 =>
+    { R: @mkCoh2PaintingTypes p k.+1 depsCohs2.(1)%depscohs2
+        (depsCohs2; extraDepsCohs2)%extradepscohs2 &T
+         mkCoh2PaintingType depsCohs2 extraDepsCohs2 }
+  end.
+
+Arguments mkCoh2PaintingTypes {p k depsCohs2} extraDepsCohs2.
+
+Definition mkCoh2LayerFrameEndpointType {p k}
+  (depsCohs2: DepsCohs2 p.+1 k)
+  (extraDepsCohs2: DepsCohs2Extension p.+1 k depsCohs2)
+  (coh2Frames: mkCoh2FrameTypes (mkCohPaintings (depsCohs2; extraDepsCohs2)))
+  q (Hq: q <= k) r (Hr: r <= q) s (Hs: s <= r)
+  (d: mkFrame (mkDepsRestr (depsCohs := toDepsCohs (mkCohFrames
+    (mkCohPaintings (depsCohs2; extraDepsCohs2)).1 coh2Frames.1).1)).(1)): Type :=
+  mkRestrFrames.2 q.+1 (⇑ Hq)
+    (mkRestrFrames.2 r.+1 (⇑ (Hr ↕ ↑ Hq))
+      (mkRestrFrames.2 s.+1 (⇑ (Hs ↕ ↑ (Hr ↕ ↑ Hq))) d)) =
+  (mkRestrFrames.2 s.+1 (⇑ (Hs ↕ (Hr ↕ Hq)))
+    (mkRestrFrames.2 r.+2 (⇑ (⇑ Hr ↕ ⇑ Hq))
+      (mkRestrFrames.2 q.+3 (⇑ (⇑ (⇑ Hq))) d))).
+
+Definition mkCoh2LayerEndpointType {p k}
+  (depsCohs2: DepsCohs2 p.+1 k)
+  (extraDepsCohs2: DepsCohs2Extension p.+1 k depsCohs2)
+  (prevCoh2Frames: mkCoh2FrameTypes (mkCohPaintings (depsCohs2; extraDepsCohs2)))
+  q (Hq: q <= k) r (Hr: r <= q) s (Hs: s <= r)
+  (d: mkFrame (mkDepsRestr (depsCohs := toDepsCohs (mkCohFrames
+    (mkCohPaintings (depsCohs2; extraDepsCohs2)).1 prevCoh2Frames.1).1)).(1))
+  (l: mkLayer (mkDepsRestr (depsCohs := toDepsCohs (mkCohFrames
+    (mkCohPaintings (depsCohs2; extraDepsCohs2)).1 prevCoh2Frames.1).1)).(_restrFrames).2 d)
+  (coh2FrameEndpoint: mkCoh2LayerFrameEndpointType depsCohs2
+    extraDepsCohs2 prevCoh2Frames q Hq r Hr s Hs d): Type :=
+  let depsCohs := depsCohs2.(_depsCohs) in
+  let cohFrame1 := mkCohFrame depsCohs2.(_cohPaintings).1 depsCohs2.(_coh2Frames).1 in
+  let restrPainting1 := mkRestrPainting (depsCohs; depsCohs2.(_extraDepsCohs)) in
+  let cohFrame2 := mkCohFrame (mkCohPaintings (depsCohs2; extraDepsCohs2)).1 prevCoh2Frames.1 in
+  let restrPainting2 := mkRestrPainting ((mkDepsCohs depsCohs2).(1);
+    (mkDepsCohs depsCohs2; mkExtraCohs extraDepsCohs2)) in
+  rew [mkLayer depsCohs.(_deps).(_restrFrames).2] coh2FrameEndpoint in
+  mkRestrLayer depsCohs.(_restrPaintings).2 depsCohs.(_cohs).2 q Hq
+    (mkRestrFrame r.+1 (⇑ (Hr ↕ ↑ Hq))
+      (mkRestrFrame s.+1 (⇑ (Hs ↕ ↑ (Hr ↕ ↑ Hq))) d))
+    (mkRestrLayer restrPainting1 cohFrame1 r (Hr ↕ ↑ Hq)
+      (mkRestrFrame s.+1 (⇑ (Hs ↕ ↑ (Hr ↕ ↑ Hq))) d)
+      (mkRestrLayer restrPainting2 cohFrame2 s (Hs ↕ ↑ (Hr ↕ ↑ Hq)) d l)) =
+  mkRestrLayer depsCohs.(_restrPaintings).2 depsCohs.(_cohs).2 s (Hs ↕ (Hr ↕ Hq))
+    (mkRestrFrame r.+2 (⇑ (⇑ Hr ↕ ⇑ Hq))
+      (mkRestrFrame q.+3 (⇑ (⇑ (⇑ Hq))) d))
+    (mkRestrLayer restrPainting1 cohFrame1 r.+1 (⇑ Hr ↕ ⇑ Hq)
+      (mkRestrFrame q.+3 (⇑ (⇑ (⇑ Hq))) d)
+      (mkRestrLayer restrPainting2 cohFrame2 q.+2 (⇑ (⇑ Hq)) d l)).
+
+Definition mkCoh2LayerType {p k}
+  (depsCohs2: DepsCohs2 p.+1 k)
+  (extraDepsCohs2: DepsCohs2Extension p.+1 k depsCohs2)
+  (prevCoh2Frames: mkCoh2FrameTypes (mkCohPaintings (depsCohs2;extraDepsCohs2)))
+  q (Hq: q <= k) r (Hr: r <= q) s (Hs: s <= r)
+  (d: mkFrame (mkDepsRestr (depsCohs := toDepsCohs (mkCohFrames
+    (mkCohPaintings (depsCohs2; extraDepsCohs2)).1 prevCoh2Frames.1).1)).(1))
+  (l: mkLayer (mkDepsRestr (depsCohs := toDepsCohs (mkCohFrames (mkCohPaintings
+    (depsCohs2; extraDepsCohs2)).1 prevCoh2Frames.1).1)).(_restrFrames).2 d): Type :=
+  let depsCohs := depsCohs2.(_depsCohs) in
+  let depsCohs' := toDepsCohs (mkCohFrames
+    (mkCohPaintings (depsCohs2; extraDepsCohs2)).1 prevCoh2Frames.1) in
+  rew [mkCoh2LayerEndpointType depsCohs2 extraDepsCohs2 prevCoh2Frames q Hq r Hr s Hs d l]
+    prevCoh2Frames.2 q.+1 (⇑ Hq) r.+1 (⇑ Hr) s.+1 (⇑ Hs) d in
+  (sigT_map_eq (Q := fun x => GDom (mkLayer depsCohs.(_deps).(_restrFrames).2 x))
+    (mkRestrLayer depsCohs2.(_depsCohs).(_restrPaintings).2
+      depsCohs2.(_depsCohs).(_cohs).2 q Hq)
+    (mkCohLayer (mkCohPaintings extraDepsCohs2).1.2
+      prevCoh2Frames.2 r (Hr ↕ ↑ Hq) s Hs d l)
+  ⊙ (mkCohLayer depsCohs2.(_cohPaintings).2
+    depsCohs2.(_coh2Frames).2 q Hq s (Hs ↕ Hr)
+      (mkRestrFrame (depsCohs := depsCohs') r.+1 (⇑ (Hr ↕ ↑ Hq)) (d; l)).1
+      (mkRestrFrame (depsCohs := depsCohs') r.+1 (⇑ (Hr ↕ ↑ Hq)) (d; l)).2
+  ⊙[fun x => GDom (mkLayer depsCohs.(_deps).(_restrFrames).2 x)]
+    sigT_map_eq (Q := fun x => GDom (mkLayer depsCohs.(_deps).(_restrFrames).2 x))
+      (mkRestrLayer depsCohs2.(_depsCohs).(_restrPaintings).2
+        depsCohs2.(_depsCohs).(_cohs).2 s (Hs ↕ (Hr ↕ Hq)))
+      (mkCohLayer (mkCohPaintings extraDepsCohs2).1.2 prevCoh2Frames.2
+        q.+1 (⇑ Hq) r.+1 (⇑ Hr) d l))) =
+  mkCohLayer depsCohs2.(_cohPaintings).2
+    depsCohs2.(_coh2Frames).2 q Hq r Hr
+    (mkRestrFrame (depsCohs := depsCohs') s (↑ (↑ (Hs ↕ (Hr ↕ Hq)))) (d; l)).1
+    (mkRestrFrame (depsCohs := depsCohs') s (↑ (↑ (Hs ↕ (Hr ↕ Hq)))) (d; l)).2
+  ⊙[fun x => GDom (mkLayer depsCohs.(_deps).(_restrFrames).2 x)]
+    (sigT_map_eq (Q := fun x => GDom (mkLayer depsCohs.(_deps).(_restrFrames).2 x))
+      (mkRestrLayer depsCohs2.(_depsCohs).(_restrPaintings).2
+        depsCohs2.(_depsCohs).(_cohs).2 r (Hr ↕ Hq))  
+      (mkCohLayer (mkCohPaintings extraDepsCohs2).1.2 
+        prevCoh2Frames.2 q.+1 (⇑ Hq) s (↑ (Hs ↕ Hr)) d l)
+  ⊙ mkCohLayer depsCohs2.(_cohPaintings).2
+      depsCohs2.(_coh2Frames).2 r (Hr ↕ Hq) s Hs
+      (mkRestrFrame (depsCohs := depsCohs') q.+2 (⇑ (⇑ Hq)) (d; l)).1
+      (mkRestrFrame (depsCohs := depsCohs') q.+2 (⇑ (⇑ Hq)) (d; l)).2).
+
+Definition mkCoh2Layer {p k}
+  (depsCohs2: DepsCohs2 p.+1 k)
+  (extraDepsCohs2: DepsCohs2Extension p.+1 k depsCohs2)
+  (prevCoh2Frames: mkCoh2FrameTypes (mkCohPaintings (depsCohs2;extraDepsCohs2)))
+  (coh2Painting: mkCoh2PaintingType depsCohs2 extraDepsCohs2)
+  (* coh3Frame: mkCoh3FrameType ... - not needed as for HGpd is given by GUIP *)
+  q (Hq: q <= k) r (Hr: r <= q) s (Hs: s <= r)
+  (d: mkFrame (mkDepsRestr (depsCohs := toDepsCohs (mkCohFrames
+    (mkCohPaintings (depsCohs2; extraDepsCohs2)).1 prevCoh2Frames.1).1)).(1))
+  (l: mkLayer (mkDepsRestr (depsCohs := toDepsCohs (mkCohFrames
+    (mkCohPaintings (depsCohs2; extraDepsCohs2)).1 prevCoh2Frames.1).1)).(_restrFrames).2 d):
+  mkCoh2LayerType depsCohs2 extraDepsCohs2 prevCoh2Frames q Hq r Hr s Hs d l.
+Proof.
+  unfold mkCoh2LayerType, mkCohLayer.
+  eapply rew_coh2Layer with
+    (S1 := fun x => (mkDepsRestr (depsCohs := (mkDepsCohs depsCohs2).(1).(1))).(_paintings).2 x)
+    (S0 := fun x => (mkDepsCohs depsCohs2).(1).(_deps).(_paintings).2 x)
+    (PA := fun x => depsCohs2.(_depsCohs).(_deps).(_paintings).2 x)
+    (g0 := fun x => (mkDepsCohs depsCohs2).(1).(_deps).(_restrFrames).2 0 leR_O x)
+    (f0 := fun x => depsCohs2.(_depsCohs).(_deps).(_restrFrames).2 0 leR_O x)
+    (Rr := (mkDepsCohs depsCohs2).(1).(_restrPaintings).2 r (Hr ↕ ↑ Hq))
+    (Rs := (mkDepsCohs depsCohs2).(1).(_restrPaintings).2 s (Hs ↕ (Hr ↕ ↑ Hq)))
+    (Rq1 := (mkDepsCohs depsCohs2).(1).(_restrPaintings).2 q.+1 (⇑ Hq))
+    (Rr1 := (mkDepsCohs depsCohs2).(1).(_restrPaintings).2 r.+1 (⇑ Hr ↕ ⇑ Hq))
+    (Fq := depsCohs2.(_depsCohs).(_restrPaintings).2 q Hq)
+    (Fr := depsCohs2.(_depsCohs).(_restrPaintings).2 r (Hr ↕ Hq))
+    (Fs := depsCohs2.(_depsCohs).(_restrPaintings).2 s ((Hs ↕ Hr) ↕ Hq))
+    (gq := fun x => depsCohs2.(_depsCohs).(_cohs).2 q Hq 0 leR_O x)
+    (gr := fun x => depsCohs2.(_depsCohs).(_cohs).2 r (Hr ↕ Hq) 0 leR_O x)
+    (gs := fun x => depsCohs2.(_depsCohs).(_cohs).2 s ((Hs ↕ Hr) ↕ Hq) 0 leR_O x)
+    (KA2 := fun x => depsCohs2.(_depsCohs).(_cohs).2 q Hq s (Hs ↕ Hr) x)
+    (KA4 := fun x => depsCohs2.(_depsCohs).(_cohs).2 q Hq r Hr x)
+    (KA6 := fun x => depsCohs2.(_depsCohs).(_cohs).2 r (Hr ↕ Hq) s Hs x)
+    (HKA2 := fun x c => depsCohs2.(_cohPaintings).2 q Hq s (Hs ↕ Hr) x c)
+    (HKA4 := fun x c => depsCohs2.(_cohPaintings).2 q Hq r Hr x c)
+    (HKA6 := fun x c => depsCohs2.(_cohPaintings).2 r (Hr ↕ Hq) s Hs x c).
+  - now exact (coh2Painting q Hq r Hr s Hs
+      (((mkCohFrameTypesAndRestrFrames
+          (mkRestrPaintings (mkDepsCohs depsCohs2; mkExtraCohs extraDepsCohs2)).1.1)
+        .(RestrFramesDef) ((mkCoh2FrameTypesAndCohFrames
+            (mkCohPaintings (depsCohs2; extraDepsCohs2)).1)
+          .(CohFramesDef) prevCoh2Frames.1).1).2 0 leR_O d) l).
+  - now apply depsCohs2.(_depsCohs).(_deps).(_frames).2.(GUIP).
+Defined.
+
+Fixpoint mkCoh2Frames `{depsCohs2: DepsCohs2 p k}
+  (extraDepsCohs2: DepsCohs2Extension p k depsCohs2)
+  (coh2Paintings: mkCoh2PaintingTypes extraDepsCohs2):
+  mkCoh2FrameTypes (mkCohPaintings extraDepsCohs2).
+Proof.
+  destruct p.
+  - unshelve esplit.
+    + now exact tt.
+    + intros q Hq r Hr s Hs d.
+      now trivial.
+  - set (h := mkCoh2Frames p k.+1 depsCohs2.(1)%depscohs2
+      (depsCohs2; extraDepsCohs2)%extradepscohs2 coh2Paintings.1).
+    unshelve esplit.
+    + now exact h.
+    + intros q Hq r Hr s Hs [d l].
+      unshelve eapply eq_existT_curried_hex.
+      * now exact (h.2 q.+1 (⇑ Hq) r.+1 (⇑ Hr) s.+1 (⇑ Hs) d).
+      * now exact_no_check (mkCoh2Layer depsCohs2 extraDepsCohs2 h
+          coh2Paintings.2 q Hq r Hr s Hs d l).
+Defined.
+
+Class DepsCohs3 p k := {
+  _depsCohs2: DepsCohs2 p k;
+  _extraDepsCohs2: DepsCohs2Extension p k _depsCohs2;
+  _coh2Paintings: mkCoh2PaintingTypes _extraDepsCohs2;
+}.
+
+#[local]
+Instance toDepsCohs3 `{extraDepsCohs2: DepsCohs2Extension p k depsCohs2}
+  (coh2Paintings: mkCoh2PaintingTypes extraDepsCohs2): DepsCohs3 p k :=
+  {| _coh2Paintings := coh2Paintings |}.
+
+#[local]
+Instance proj1DepsCohs3 `(depsCohs3: DepsCohs3 p.+1 k): DepsCohs3 p k.+1 :=
+{|
+  _depsCohs2 := depsCohs3.(_depsCohs2).(1);
+  _extraDepsCohs2 := (depsCohs3.(_depsCohs2); depsCohs3.(_extraDepsCohs2));
+  _coh2Paintings := depsCohs3.(_coh2Paintings).1;
+|}.
+
+Declare Scope depscohs3_scope.
+Delimit Scope depscohs3_scope with depscohs3.
+Bind Scope depscohs3_scope with DepsCohs3.
+Notation "x .(1)" := (proj1DepsCohs3 x%depscohs3)
+  (at level 1, left associativity, format "x .(1)"): depscohs3_scope.
+
+#[local]
+Instance mkDepsCohs2 `(depsCohs3: DepsCohs3 p k): DepsCohs2 p.+1 k :=
+{|
+  _depsCohs := mkDepsCohs depsCohs3.(_depsCohs2);
+  _extraDepsCohs := mkExtraCohs depsCohs3.(_extraDepsCohs2);
+  _cohPaintings := mkCohPaintings depsCohs3.(_extraDepsCohs2);
+  _coh2Frames := mkCoh2Frames depsCohs3.(_extraDepsCohs2) depsCohs3.(_coh2Paintings);
+|}.
+
+Inductive DepsCohs3Extension p: forall k (depsCohs3: DepsCohs3 p k), Type :=
+| TopCoh3Dep `{depsCohs3: DepsCohs3 p 0}
+  (E: mkFrame (mkDepsRestr (depsCohs := mkDepsCohs (mkDepsCohs2 depsCohs3))) -> HGpd)
+  : DepsCohs3Extension p 0 depsCohs3
+| AddCoh3Dep {k} (depsCohs3: DepsCohs3 p.+1 k):
+  DepsCohs3Extension p.+1 k depsCohs3 ->
+  DepsCohs3Extension p k.+1 depsCohs3.(1).
+
+Arguments TopCoh3Dep {p depsCohs3}.
+Arguments AddCoh3Dep {p k}.
+
+Declare Scope extra_depscohs3_scope.
+Delimit Scope extra_depscohs3_scope with extradepscohs3.
+Bind Scope extra_depscohs3_scope with DepsCohs3Extension.
+Notation "( x ; y )" := (AddCoh3Dep x y)
+  (at level 0, format "( x ; y )"): extra_depscohs3_scope.
+
+Fixpoint mkExtraCohs2 `{depsCohs3: DepsCohs3 p k}
+  (extraDepsCohs3: DepsCohs3Extension p k depsCohs3):
+  DepsCohs2Extension p.+1 k (mkDepsCohs2 depsCohs3).
+Proof.
+  destruct extraDepsCohs3.
+  - now constructor.
+  - apply (AddCoh2Dep (mkDepsCohs2 depsCohs3)).
+    now exact (mkExtraCohs2 p.+1 k depsCohs3 extraDepsCohs3).
+Defined.
+
+Definition mkCoh2Painting `{depsCohs3: DepsCohs3 p k}
+  (extraDepsCohs3: DepsCohs3Extension p k depsCohs3):
+  mkCoh2PaintingType (mkDepsCohs2 depsCohs3) (mkExtraCohs2 extraDepsCohs3).
+Proof.
+  intros q Hq r Hr s.
+  generalize dependent r.
+  generalize dependent q.
+  generalize dependent k.
+  generalize dependent p.
+  induction s as [|s mkCoh2Painting].
+  - intros p k depsCohs3 extraDepsCohs3 q Hq r Hr Hs d c.
+    unfold mkCoh2PaintingInstanceType; cbn.
+    unfold mkCohLayer.
+    now apply rew_coh2Painting_restr0 with
+      (P := fun x : (mkDepsCohs depsCohs3.(_depsCohs2)).(_deps).(_frames).2 =>
+        (mkDepsCohs depsCohs3.(_depsCohs2)).(_deps).(_paintings).2 x)
+      (rf0 := fun x =>
+        (mkDepsCohs depsCohs3.(_depsCohs2)).(_deps).(_restrFrames).2 0 leR_O x)
+      (F := (mkDepsCohs depsCohs3.(_depsCohs2)).(_restrPaintings).2 q Hq)
+      (G := (mkDepsCohs depsCohs3.(_depsCohs2)).(_restrPaintings).2 r (Hr ↕ Hq))
+      (R0 := fun z => mkPainting (mkExtraDeps depsCohs3.(_depsCohs2).(_extraDepsCohs)) z)
+      (HH := (mkCoh2Frames depsCohs3.(_extraDepsCohs2)
+        depsCohs3.(_coh2Paintings)).2 q Hq r Hr 0 leR_O d)
+      (HK := mkCohPainting depsCohs3.(_extraDepsCohs2) q Hq r Hr _ c.1).
+  - intros p k depsCohs3 extraDepsCohs3 q Hq r Hr Hs d c.
+    destruct r; [now contradiction |].
+    destruct q; [now contradiction |].
+    destruct extraDepsCohs3; [now contradiction |].
+    destruct c as [l c].
+    unfold mkCoh2PaintingInstanceType; cbv zeta.
+    set (Q := mkCoh2PaintingEndpointType _ _ q.+1 Hq r.+1 Hr s.+1 Hs d (l; c)).
+    set (H := (mkDepsCohs2 depsCohs3.(1)).(_coh2Frames).2 q.+1 Hq r.+1 Hr s.+1 Hs d).
+    cbn [mkDepsCohs2 _cohPaintings mkCohPaintings projT2].
+    unfold mkCohPainting; cbn [nat_ind].
+    change (depsCohs3.(1).(_extraDepsCohs2)) with
+      (AddCoh2Dep depsCohs3.(_depsCohs2) depsCohs3.(_extraDepsCohs2)).
+    lazy beta iota.
+    unshelve eapply (eq_existT_curried_dep_hex
+      (A0 := ((mkRestrFrameTypesAndFrames
+          (mkDepsCohs2 depsCohs3.(1)).(_depsCohs).(_deps).(_paintings).1)
+        .(FrameDef)
+          (mkDepsCohs2 depsCohs3.(1)).(_depsCohs).(_deps).(_restrFrames).1).2)
+      (B := ((mkRestrFrameTypesAndFrames
+          depsCohs3.(_depsCohs2).(_depsCohs).(_deps).(_paintings).1)
+        .(FrameDef)
+          depsCohs3.(_depsCohs2).(_depsCohs).(_deps).(_restrFrames).1).2)
+      (P0 := fun a => (mkLayer
+        (mkDepsCohs2 depsCohs3.(1)).(_depsCohs).(_deps).(_restrFrames).2
+        a).(GDom))
+      (R0 := fun a u => (mkPainting
+        (mkDepsCohs2 depsCohs3.(1)).(_depsCohs).(_extraDeps) (a; u)).(GDom))
+      (P' := fun b => (mkLayer
+        depsCohs3.(_depsCohs2).(_depsCohs).(_deps).(_restrFrames).2 b).(GDom))
+      (R' := fun b u => (mkPainting
+        depsCohs3.(_depsCohs2).(_depsCohs).(_extraDeps) (b; u)).(GDom))
+      ((mkDepsCohs2 depsCohs3.(1)).(_depsCohs).(_deps).(_restrFrames).2
+        q.+1 Hq)
+      (fun d0 l0 => mkRestrLayer
+        depsCohs3.(_depsCohs2).(_depsCohs).(_restrPaintings).2
+        depsCohs3.(_depsCohs2).(_depsCohs).(_cohs).2 q (⇓ Hq) d0 l0)
+      (fun d0 l0 c0 => mkRestrPainting
+        depsCohs3.(_depsCohs2).(_extraDepsCohs) q (⇓ Hq) (d0; l0) c0)
+      ((mkDepsCohs2 depsCohs3.(1)).(_depsCohs).(_deps).(_restrFrames).2
+        s.+1 (Hs ↕ (Hr ↕ Hq)))
+      (fun d0 l0 => mkRestrLayer
+        depsCohs3.(_depsCohs2).(_depsCohs).(_restrPaintings).2
+        depsCohs3.(_depsCohs2).(_depsCohs).(_cohs).2
+        s (⇓ (Hs ↕ (Hr ↕ Hq))) d0 l0)
+      (fun d0 l0 c0 => mkRestrPainting
+        depsCohs3.(_depsCohs2).(_extraDepsCohs)
+        s (⇓ (Hs ↕ (Hr ↕ Hq))) (d0; l0) c0)
+      ((mkDepsCohs2 depsCohs3.(1)).(_depsCohs).(_deps).(_restrFrames).2
+        r.+1 (Hr ↕ Hq))
+      (fun d0 l0 => mkRestrLayer
+        depsCohs3.(_depsCohs2).(_depsCohs).(_restrPaintings).2
+        depsCohs3.(_depsCohs2).(_depsCohs).(_cohs).2 r (⇓ (Hr ↕ Hq)) d0 l0)
+      (fun d0 l0 c0 => mkRestrPainting
+        depsCohs3.(_depsCohs2).(_extraDepsCohs) r (⇓ (Hr ↕ Hq)) (d0; l0) c0)).
+    + now exact (mkCoh2Layer depsCohs3.(_depsCohs2) depsCohs3.(_extraDepsCohs2)
+        (mkCoh2Frames (depsCohs3.(_depsCohs2); depsCohs3.(_extraDepsCohs2))
+          depsCohs3.(1).(_coh2Paintings))
+        depsCohs3.(_coh2Paintings).2 q (⇓ Hq) r (⇓ Hr) s (⇓ Hs) d l).
+    + now exact_no_check (mkCoh2Painting p.+1 k depsCohs3 extraDepsCohs3
+        q (⇓ Hq) r (⇓ Hr) (⇓ Hs) (d; l) c).
+Defined.
+
+Fixpoint mkCoh2Paintings `{depsCohs3: DepsCohs3 p k}
+  (extraDepsCohs3: DepsCohs3Extension p k depsCohs3) {struct p}:
+  mkCoh2PaintingTypes (mkExtraCohs2 extraDepsCohs3).
+Proof.
+  destruct p.
+  - unshelve esplit. now exact tt.
+    now exact (mkCoh2Painting extraDepsCohs3).
+  - unshelve esplit. now exact (mkCoh2Paintings p k.+1
+      depsCohs3.(1)%depscohs3 (depsCohs3; extraDepsCohs3)%extradepscohs3).
+    now exact (mkCoh2Painting extraDepsCohs3).
+Defined.
+
+(** The data of a semi-simplicial groupoid truncated in dimension p,
+    as in νSet, with the two additional levels of coherence data ([coh2Frames],
+    [coh2Paintings]) that UIP provided for free at the [HSet] level *)
+
+Class SSGpdData p := {
+  frames: mkFrameTypes p 0;
+  paintings: mkPaintingTypes p 0 frames;
+  restrFrames: mkRestrFrameTypes paintings;
+  restrPaintings E: mkRestrPaintingTypes (TopRestrDep E);
+  cohFrames E: mkCohFrameTypes (restrPaintings E);
+  cohPaintings E E': mkCohPaintingTypes
+    (depsCohs := toDepsCohs (deps := toDepsRestr restrFrames) (cohFrames E))
+    (TopCohDep E');
+  coh2Frames E E': mkCoh2FrameTypes (cohPaintings E E');
+  coh2Paintings E E' E'': mkCoh2PaintingTypes
+    (depsCohs2 := toDepsCohs2 (coh2Frames E E'))
+    (TopCoh2Dep E'');
+}.
+
+Section SSGpdData.
+Variable p: nat.
+Variable C: SSGpdData p.
+Variable E: mkFrame (toDepsRestr C.(restrFrames)) -> HGpd.
+
+#[local]
+Instance mkSSGpdData: SSGpdData p.+1 :=
+{|
+  frames := mkFrames _;
+  paintings := mkPaintings _;
+  restrFrames := mkRestrFrames;
+  restrPaintings E' := mkRestrPaintings (TopCohDep E');
+  cohFrames E' := mkCohFrames (C.(cohPaintings) E E') (C.(coh2Frames) E E');
+  cohPaintings E' E'' := mkCohPaintings
+    (TopCoh2Dep (depsCohs2 := toDepsCohs2 (C.(coh2Frames) E E')) E'');
+  coh2Frames E' E'' := mkCoh2Frames
+    (TopCoh2Dep (depsCohs2 := toDepsCohs2 (C.(coh2Frames) E E')) E'')
+    (C.(coh2Paintings) E E' E'');
+  coh2Paintings E' E'' E''' := mkCoh2Paintings
+    (TopCoh3Dep (depsCohs3 := toDepsCohs3 (C.(coh2Paintings) E E' E'')) E''');
+|}.
+End SSGpdData.
+
+Class SSGpd p := {
+  prefix: Type;
+  data: prefix -> SSGpdData p;
+}.
+
+(** ************************************************)
+(** The construction of [SSGpd n+1] from [SSGpd n] *)
+
+(** Extending the initial prefix *)
+Definition mkPrefix p {C: SSGpd p}: Type :=
+  { D: C.(prefix) &T mkFrame (toDepsRestr (C.(data) D).(restrFrames)) -> HGpd }.
+
+#[local]
+Instance mkSSGpd0: SSGpd 0.
+Proof.
+  unshelve esplit.
+  - now exact gunit.
+  - unshelve esplit; now trivial.
+Defined.
+
+#[local]
+Instance mkSSGpd {p} (C: SSGpd p): SSGpd p.+1 :=
+{|
+  prefix := mkPrefix p;
+  data := fun D: mkPrefix p => mkSSGpdData p (C.(data) D.1) D.2;
+|}.
+
+(** An [SSGpd] truncated up to dimension [n] *)
+Fixpoint SSGpdAt n: SSGpd n :=
+  match n with
+  | O => mkSSGpd0
+  | n.+1 => mkSSGpd (SSGpdAt n)
+  end.
+
+CoInductive SSGpdFrom n (X: (SSGpdAt n).(prefix)): Type := cons {
+  this: mkFrame (toDepsRestr ((SSGpdAt n).(data) X).(restrFrames)) -> HGpd;
+  next: SSGpdFrom n.+1 (X; this);
+}.
+
+(** The final construction *)
+Definition SSGpds := SSGpdFrom 0 tt.
+
+End SSGpd.
+
+(** Some example *)
+
+Example SemiSimplicial5 := Eval lazy in (SSGpd.SSGpdAt 5).(SSGpd.prefix _).
+Print SemiSimplicial5.
