theories/νSet/SSGpdLemmas.v
@@ -1,0 +1,465 @@
+Set Warnings "-notation-overridden".
+From Bonak Require Import SigT Notation.
+
+Set Keyed Unification.
+
+Lemma eq_existT_curried_hex {A1 A2 A3 B: Type}
+  {P1: A1 -> Type} {P2: A2 -> Type} {P3: A3 -> Type} {Q: B -> Type}
+  (f1: A1 -> B) (g1: forall a, P1 a -> Q (f1 a))
+  (f2: A2 -> B) (g2: forall a, P2 a -> Q (f2 a))
+  (f3: A3 -> B) (g3: forall a, P3 a -> Q (f3 a))
+  {x1 y1: A1} {u1: P1 x1} {v1: P1 y1}
+  {x2 y2: A2} {u2: P2 x2} {v2: P2 y2}
+  {x3 y3: A3} {u3: P3 x3} {v3: P3 y3}
+  {K1: x1 = y1} {W1: rew [P1] K1 in u1 = v1}
+  {K2: x2 = y2} {W2: rew [P2] K2 in u2 = v2}
+  {K3: x3 = y3} {W3: rew [P3] K3 in u3 = v3}
+  {H2: f1 y1 = f3 x3} {U2: rew [Q] H2 in g1 y1 v1 = g3 x3 u3}
+  {H1': f1 x1 = f2 x2} {U1': rew [Q] H1' in g1 x1 u1 = g2 x2 u2}
+  {H3': f2 y2 = f3 y3} {U3': rew [Q] H3' in g2 y2 v2 = g3 y3 v3}
+  (HH: f_equal f1 K1 • (H2 • f_equal f3 K3) =
+    H1' • (f_equal f2 K2 • H3'))
+  (HHu: rew [fun h => rew [Q] h in g1 x1 u1 = g3 y3 v3] HH in
+    (sigT_map_eq g1 W1 ⊙ (U2 ⊙ sigT_map_eq g3 W3)) =
+    U1' ⊙ (sigT_map_eq g2 W2 ⊙ U3')):
+  f_equal (fun z: {a: A1 &T P1 a} => (f1 z.1; g1 z.1 z.2)) (= K1; W1)
+  • ((= H2; U2)
+     • f_equal (fun z: {a: A3 &T P3 a} => (f3 z.1; g3 z.1 z.2)) (= K3; W3)) =
+  (= H1'; U1')
+  • (f_equal (fun z: {a: A2 &T P2 a} => (f2 z.1; g2 z.1 z.2)) (= K2; W2)
+     • (= H3'; U3')).
+Proof.
+  rewrite 3 f_equal_eq_existT_curried.
+  rewrite 4 eq_trans_eq_existT_curried.
+  now exact (eq_existT_curried_eq HH HHu).
+Defined.
+
+Lemma eq_existT_curried_dep_hex
+  {A0 B: Type} {P0: A0 -> Type} {R0: forall a, P0 a -> Type}
+  {P': B -> Type} {R': forall b, P' b -> Type}
+  (f1: A0 -> B) (g1: forall a, P0 a -> P' (f1 a))
+  (h1: forall a u, R0 a u -> R' (f1 a) (g1 a u))
+  (f3: A0 -> B) (g3: forall a, P0 a -> P' (f3 a))
+  (h3: forall a u, R0 a u -> R' (f3 a) (g3 a u))
+  (f2: A0 -> B) (g2: forall a, P0 a -> P' (f2 a))
+  (h2: forall a u, R0 a u -> R' (f2 a) (g2 a u))
+  {x0 x1 x2 x3 x1' x2': A0}
+  {u0: P0 x0} {v0: R0 x0 u0} {u1: P0 x1} {v1: R0 x1 u1}
+  {u2: P0 x2} {v2: R0 x2 u2} {u3: P0 x3} {v3: R0 x3 u3}
+  {u1': P0 x1'} {v1': R0 x1' u1'} {u2': P0 x2'} {v2': R0 x2' u2'}
+  (H1: x0 = x1) (Hu1: rew [P0] H1 in u0 = u1)
+  (Hv1: rew [fun z => R0 z.1 z.2] (=H1; Hu1) in
+    (v0: (fun z => R0 z.1 z.2) (x0; u0)) = v1)
+  (H2: f1 x1 = f3 x2) (Hu2: rew [P'] H2 in g1 x1 u1 = g3 x2 u2)
+  (Hv2: rew [fun z => R' z.1 z.2] (=H2; Hu2) in
+    (h1 x1 u1 v1: (fun z => R' z.1 z.2) (f1 x1; g1 x1 u1)) = h3 x2 u2 v2)
+  (H3: x2 = x3) (Hu3: rew [P0] H3 in u2 = u3)
+  (Hv3: rew [fun z => R0 z.1 z.2] (=H3; Hu3) in
+    (v2: (fun z => R0 z.1 z.2) (x2; u2)) = v3)
+  (H1': f1 x0 = f2 x1') (Hu1': rew [P'] H1' in g1 x0 u0 = g2 x1' u1')
+  (Hv1': rew [fun z => R' z.1 z.2] (=H1'; Hu1') in
+    (h1 x0 u0 v0: (fun z => R' z.1 z.2) (f1 x0; g1 x0 u0)) = h2 x1' u1' v1')
+  (H2': x1' = x2') (Hu2': rew [P0] H2' in u1' = u2')
+  (Hv2': rew [fun z => R0 z.1 z.2] (=H2'; Hu2') in
+    (v1': (fun z => R0 z.1 z.2) (x1'; u1')) = v2')
+  (H3': f2 x2' = f3 x3) (Hu3': rew [P'] H3' in g2 x2' u2' = g3 x3 u3)
+  (Hv3': rew [fun z => R' z.1 z.2] (=H3'; Hu3') in
+    (h2 x2' u2' v2': (fun z => R' z.1 z.2) (f2 x2'; g2 x2' u2')) = h3 x3 u3 v3)
+  (HH: f_equal f1 H1 • (H2 • f_equal f3 H3) =
+    H1' • (f_equal f2 H2' • H3'))
+  (HHu: rew [fun h => rew [P'] h in g1 x0 u0 = g3 x3 u3] HH in
+    (sigT_map_eq g1 Hu1 ⊙ (Hu2 ⊙ sigT_map_eq g3 Hu3)) =
+    Hu1' ⊙ (sigT_map_eq g2 Hu2' ⊙ Hu3'))
+  (HHv:
+    rew [fun p: (f1 x0; g1 x0 u0) = (f3 x3; g3 x3 u3) =>
+        rew [fun z: {a: B &T P' a} => R' z.1 z.2] p in
+        (h1 x0 u0 v0:
+          (fun z: {a: B &T P' a} => R' z.1 z.2) (f1 x0; g1 x0 u0)) =
+        h3 x3 u3 v3]
+      eq_existT_curried_hex f1 g1 f2 g2 f3 g3 HH HHu in
+    (@sigT_map_eq _ _ (fun z: {x: A0 &T P0 x} => R0 z.1 z.2)
+       (fun z: {x: B &T P' x} => R' z.1 z.2)
+       (fun z => (f1 z.1; g1 z.1 z.2)) (fun z => h1 z.1 z.2)
+       (x0; u0) (x1; u1) v0 v1 (=H1; Hu1) Hv1
+     ⊙ (Hv2
+        ⊙ @sigT_map_eq _ _ (fun z: {x: A0 &T P0 x} => R0 z.1 z.2)
+            (fun z: {x: B &T P' x} => R' z.1 z.2)
+            (fun z => (f3 z.1; g3 z.1 z.2)) (fun z => h3 z.1 z.2)
+            (x2; u2) (x3; u3) v2 v3 (=H3; Hu3) Hv3)) =
+    Hv1'
+    ⊙ (@sigT_map_eq _ _ (fun z: {x: A0 &T P0 x} => R0 z.1 z.2)
+         (fun z: {x: B &T P' x} => R' z.1 z.2)
+         (fun z => (f2 z.1; g2 z.1 z.2)) (fun z => h2 z.1 z.2)
+         (x1'; u1') (x2'; u2') v1' v2' (=H2'; Hu2') Hv2' ⊙ Hv3')):
+  rew [fun h => rew [fun x => {a: P' x &T R' x a}] h in
+      (g1 x0 u0; h1 x0 u0 v0) = (g3 x3 u3; h3 x3 u3 v3)] HH in
+  (sigT_map_eq (fun a uv => (g1 a uv.1; h1 a uv.1 uv.2))
+     (eq_existT_curried_dep (Q := fun z => R0 z.1 z.2)
+        (H := H1) (Hu := Hu1) (Hv := Hv1))
+   ⊙ (eq_existT_curried_dep (Q := fun z => R' z.1 z.2)
+        (H := H2) (Hu := Hu2) (Hv := Hv2)
+      ⊙ sigT_map_eq (fun a uv => (g3 a uv.1; h3 a uv.1 uv.2))
+          (eq_existT_curried_dep (Q := fun z => R0 z.1 z.2)
+             (H := H3) (Hu := Hu3) (Hv := Hv3)))) =
+  eq_existT_curried_dep (Q := fun z => R' z.1 z.2)
+    (H := H1') (Hu := Hu1') (Hv := Hv1')
+  ⊙ (sigT_map_eq (fun a uv => (g2 a uv.1; h2 a uv.1 uv.2))
+       (eq_existT_curried_dep (Q := fun z => R0 z.1 z.2)
+          (H := H2') (Hu := Hu2') (Hv := Hv2'))
+     ⊙ eq_existT_curried_dep (Q := fun z => R' z.1 z.2)
+         (H := H3') (Hu := Hu3') (Hv := Hv3')).
+Proof.
+  rewrite 3 sigT_map_eq_existT_curried_dep_curried.
+  rewrite 4 (sigT_trans_eq_existT_curried_dep (Q := fun z => R' z.1 z.2)).
+  refine (eq_existT_curried_dep_eq (Q := fun z => R' z.1 z.2) HH HHu _).
+  unfold eq_existT_curried_hex in HHv.
+  cbn [projT1 projT2] in HHv |- *.
+  revert HHv.
+  generalize (eq_existT_curried_eq HH HHu).
+  do 4 lazymatch goal with
+  | |- context [ @eq_trans_eq_existT_curried ?A ?P ?x ?y ?z ?u ?v ?w
+        ?p ?q ?p' ?q' ] =>
+      generalize (@eq_trans_eq_existT_curried A P x y z u v w p q p' q')
+  end.
+  generalize (f_equal_eq_existT_curried f2 g2 H2' Hu2').
+  generalize (f_equal_eq_existT_curried f3 g3 H3 Hu3).
+  generalize (f_equal_eq_existT_curried f1 g1 H1 Hu1).
+  generalize (= f_equal f1 H1; sigT_map_eq g1 Hu1).
+  generalize (= f_equal f3 H3; sigT_map_eq g3 Hu3).
+  generalize (= f_equal f2 H2'; sigT_map_eq g2 Hu2').
+  generalize (= H2 • f_equal f3 H3; Hu2 ⊙ sigT_map_eq g3 Hu3).
+  generalize (= f_equal f2 H2' • H3'; sigT_map_eq g2 Hu2' ⊙ Hu3').
+  generalize (= f_equal f1 H1 • (H2 • f_equal f3 H3);
+    sigT_map_eq g1 Hu1 ⊙ (Hu2 ⊙ sigT_map_eq g3 Hu3)).
+  generalize (= H1' • (f_equal f2 H2' • H3');
+    Hu1' ⊙ (sigT_map_eq g2 Hu2' ⊙ Hu3')).
+  intros qR qL q23' q23 q2' q3 q1 e e0 e1 e2 e3 e4 e5 e6.
+  destruct e, e0, e1, e2, e3, e4, e5.
+  intros HHv'; now exact HHv'.
+Defined.
+
+Lemma rew_cohLayer {T1 T2 T3 X: Type} (P: X -> Type)
+  {S2: T2 -> Type} {S3: T3 -> Type}
+  (rf0: T1 -> X) {rfF: T2 -> X} {rfG: T3 -> X}
+  (F: forall m, S2 m -> P (rfF m))
+  (G: forall n, S3 n -> P (rfG n))
+  {d1 d2: T1} (E1: d1 = d2)
+  {m1 m2: T2} (C2: m1 = m2)
+  {n1 n2: T3} (D2: n1 = n2)
+  (C1: rfF m2 = rf0 d1) (D1: rfG n2 = rf0 d2)
+  (K: rfF m1 = rfG n1)
+  (aL: S2 m1) (aR: S3 n1):
+  rew [P] K in F m1 aL = G n1 aR ->
+  f_equal rfF C2 • (C1 • f_equal rf0 E1) =
+  K • (f_equal rfG D2 • D1) ->
+  rew [fun d => P (rf0 d)] E1 in rew [P] C1 in F m2 (rew [S2] C2 in aL)
+  = rew [P] D1 in G n2 (rew [S3] D2 in aR).
+Proof.
+  intros HC Hpath.
+  rewrite <- (map_subst F C2 aL), <- (map_subst G D2 aR).
+  rewrite <- HC.
+  rewrite (rew_map P rf0 E1), (rew_map P rfF C2), (rew_map P rfG D2).
+  rewrite 4 rew_compose.
+  now exact (f_equal (fun h => rew [P] h in F m1 aL) Hpath).
+Defined.
+
+Lemma rew_coh2Painting_restr0 {Tp Td: Type} {S: Tp -> Type} (P: Td -> Type)
+  (rf0: Tp -> Td) {rfF rfG: Tp -> Td}
+  (F: forall m, S m -> P (rfF m))
+  (G: forall n, S n -> P (rfG n))
+  {d1 d2: Tp} (E1: d1 = d2)
+  {m1 m2: Tp} (C2: m1 = m2)
+  {n1 n2: Tp} (D2: n1 = n2)
+  (C1: rfF m2 = rf0 d1) (D1: rfG n2 = rf0 d2)
+  (K: rfF m1 = rfG n1)
+  (aL: S m1) (aR: S n1)
+  (HK: rew [P] K in F m1 aL = G n1 aR)
+  (HH: f_equal rfF C2 • (C1 • f_equal rf0 E1) =
+       K • (f_equal rfG D2 • D1))
+  (R0: {a: Tp &T P (rf0 a)} -> Type)
+  {v0: R0 (d1; rew [P] C1 in F m2 (rew [S] C2 in aL))}
+  {v1: R0 (d2; rew [P] D1 in G n2 (rew [S] D2 in aR))}
+  (Hv: rew [R0] (= E1; rew_cohLayer P rf0 F G E1 C2 D2 C1 D1 K aL aR HK HH)
+    in v0 = v1):
+  rew [fun π: rfF m1 = rf0 d2 =>
+      rew [P] π in F m1 aL = rew [P] D1 in G n2 (rew [S] D2 in aR)] HH in
+  (sigT_map_eq (Q := P) F (eq_refl (x := rew [S] C2 in aL))
+   ⊙ ((eq_refl : rew [P] C1 in F m2 (rew [S] C2 in aL)
+       = rew [P] C1 in F m2 (rew [S] C2 in aL))
+      ⊙ sigT_map_eq (P := fun a => {u: P (rf0 a) &T R0 (a; u)}) (Q := P)
+          (f := rf0) (fun a uv => uv.1)
+          (eq_existT_curried_dep (Q := R0) (H := E1)
+            (Hu := rew_cohLayer P rf0 F G E1 C2 D2 C1 D1 K aL aR HK HH)
+            (Hv := Hv)))) =
+  HK ⊙ (sigT_map_eq (Q := P) G (eq_refl (x := rew [S] D2 in aR)) ⊙ eq_refl).
+Proof.
+  rewrite (sigT_map_eq_existT_curried_dep_fst rf0 (fun a u => u) E1
+    (rew_cohLayer P rf0 F G E1 C2 D2 C1 D1 K aL aR HK HH) Hv).
+  cbn [projT1].
+  clear Hv v0 v1 R0.
+  destruct E1, C2, D2.
+  cbn in HH |- *.
+  revert HH. revert HK. revert C1. revert D1.
+  generalize (G n1 aR) as gb.
+  intros gb D1 C1 HK HH.
+  rewrite (sigT_map_eq_id_refl rf0).
+  revert HH. revert HK. revert C1. revert D1.
+  generalize (rf0 d1) as X.
+  intros X D1.
+  destruct D1.
+  intros C1 HK HH.
+  cbn in HH.
+  revert HK.
+  destruct HH.
+  intros HK.
+  cbn in HK |- *.
+  destruct HK.
+  revert C1.
+  generalize (rfG n1) as Y.
+  intros Y C1.
+  destruct C1.
+  now reflexivity.
+Defined.
+
+Section Coh2Layer.
+
+Variables (T1 T0 XA: Type).
+Variable S1: T1 -> Type.
+Variable S0: T0 -> Type.
+Variable PA: XA -> Type.
+
+Variables (g0 uq1 ur ur1 us hq hr hs: T1 -> T0).
+Variables (f0 fq fr fs: T0 -> XA).
+
+Variable Rr: forall x, S1 x -> S0 (ur x).
+Variable Rs: forall x, S1 x -> S0 (us x).
+Variable Rq1: forall x, S1 x -> S0 (uq1 x).
+Variable Rr1: forall x, S1 x -> S0 (ur1 x).
+Variable Fq: forall y, S0 y -> PA (fq y).
+Variable Fr: forall y, S0 y -> PA (fr y).
+Variable Fs: forall y, S0 y -> PA (fs y).
+
+Variable gq: forall x, fq (g0 x) = f0 (hq x).
+Variable gr: forall x, fr (g0 x) = f0 (hr x).
+Variable gs: forall x, fs (g0 x) = f0 (hs x).
+
+Variable KA2: forall x, fq (us x) = fs (uq1 x).
+Variable KA4: forall x, fq (ur x) = fr (uq1 x).
+Variable KA6: forall x, fr (us x) = fs (ur1 x).
+
+Variable HKA2: forall x (c: S1 x),
+  rew [PA] KA2 x in Fq (us x) (Rs x c) = Fs (uq1 x) (Rq1 x c).
+Variable HKA4: forall x (c: S1 x),
+  rew [PA] KA4 x in Fq (ur x) (Rr x c) = Fr (uq1 x) (Rq1 x c).
+Variable HKA6: forall x (c: S1 x),
+  rew [PA] KA6 x in Fr (us x) (Rs x c) = Fs (ur1 x) (Rr1 x c).
+
+(** The permutahedral coherence of frames: the hexagon proved as a
+    composition of the seven other hexagons of the permutahedron. The six
+    squares hold by naturality and don't appear here explicitly. *)
+Lemma permutahedral_coherence
+  (n1 n2 n3 m1 m2 m3 dd11 dd21 dd13 dd23 dd15 dd25: T1)
+  (b1: n1 = m1) (b2: n2 = m2) (b3: n3 = m3)
+  (KB1: ur n1 = us n2) (KB3: uq1 n2 = ur1 n3) (KB5: uq1 n1 = us n3)
+  (E11: dd11 = dd21) (E13: dd13 = dd23) (E15: dd15 = dd25)
+  (C11: ur m1 = g0 dd11) (D11: us m2 = g0 dd21)
+  (C13: uq1 m2 = g0 dd13) (D13: ur1 m3 = g0 dd23)
+  (C15: uq1 m1 = g0 dd15) (D15: us m3 = g0 dd25)
+  (E12: hq dd21 = hs dd13) (E14: hq dd11 = hr dd15)
+  (E16: hr dd25 = hs dd23)
+  (HHB1: f_equal ur b1 • (C11 • f_equal g0 E11) =
+         KB1 • (f_equal us b2 • D11))
+  (HHB3: f_equal uq1 b2 • (C13 • f_equal g0 E13) =
+         KB3 • (f_equal ur1 b3 • D13))
+  (HHB5: f_equal uq1 b1 • (C15 • f_equal g0 E15) =
+         KB5 • (f_equal us b3 • D15))
+  (HH2: f_equal fq D11 • (gq dd21 • f_equal f0 E12) =
+        KA2 m2 • (f_equal fs C13 • gs dd13))
+  (HH4: f_equal fq C11 • (gq dd11 • f_equal f0 E14) =
+        KA4 m1 • (f_equal fr C15 • gr dd15))
+  (HH6: f_equal fr D15 • (gr dd25 • f_equal f0 E16) =
+        KA6 m3 • (f_equal fs D13 • gs dd23))
+  (HHs: f_equal hq E11 • (E12 • f_equal hs E13) =
+        E14 • (f_equal hr E15 • E16)):
+  f_equal fq KB1 • (KA2 n2 • f_equal fs KB3) =
+  KA4 n1 • (f_equal fr KB5 • KA6 n3).
+Proof.
+  destruct b1, b2, b3, E11, E13, E15.
+  cbn in HHB1, HHB3, HHB5, HHs.
+  revert KB1 KB3 KB5 D11 D13 D15 C11 C13 C15 HHB1 HHB3 HHB5
+    E16 E12 E14 HHs HH2 HH4 HH6.
+  generalize (KA2 n2). generalize (KA4 n1). generalize (KA6 n3).
+  generalize (gq dd11). generalize (gs dd13). generalize (gr dd15).
+  generalize (hq dd11). generalize (hs dd13). generalize (hr dd15).
+  generalize (g0 dd11). generalize (g0 dd13). generalize (g0 dd15).
+  generalize (ur n1). generalize (us n2). generalize (uq1 n2).
+  generalize (ur1 n3). generalize (uq1 n1). generalize (us n3).
+  intros t t0 t1 t2 t3 t4 t5 t6 t7 t8 t9 t10 ge gs0 gq0 k6 k4 k2
+    KB1 KB3 KB5 D11 D13 D15 C11 C13 C15 HHB1 HHB3 HHB5
+    E16 E12 E14 HHs HH2 HH4 HH6.
+  revert ge gs0 gq0 C11 C13 C15 HHB1 HHB3 HHB5 E16 E12 E14 HHs HH2 HH4 HH6.
+  destruct D11, D13, D15.
+  intros ge gs0 gq0 C11 C13 C15 HHB1 HHB3 HHB5.
+  cbn in HHB1, HHB3, HHB5.
+  destruct HHB1, HHB3, HHB5.
+  revert ge gs0 gq0.
+  destruct C11, C13, C15.
+  intros ge gs0 gq0 E16 E12 E14 HHs.
+  revert E12 E14 HHs ge gs0 gq0.
+  destruct E16.
+  destruct E12.
+  intros E14 HHs. cbn in HHs. destruct HHs.
+  intros ge gs0 gq0.
+  revert k2 k4 k6.
+  revert gs0 ge gq0.
+  cbn.
+  generalize (fq t4). generalize (fs t2). generalize (fr t0).
+  generalize (f0 t10).
+  destruct gs0.
+  destruct ge.
+  destruct gq0.
+  intros k2 k4 k6 HH2 HH4 HH6.
+  cbn in HH2, HH4, HH6.
+  destruct HH2, HH4, HH6.
+  now reflexivity.
+Defined.
+
+Lemma rew_coh2Layer
+  (n1 n2 n3 m1 m2 m3 dd11 dd21 dd13 dd23 dd15 dd25: T1)
+  (a1: S1 n1) (a2: S1 n2) (a3: S1 n3)
+  (b1: n1 = m1) (b2: n2 = m2) (b3: n3 = m3)
+  (KB1: ur n1 = us n2) (KB3: uq1 n2 = ur1 n3) (KB5: uq1 n1 = us n3)
+  (E11: dd11 = dd21) (E13: dd13 = dd23) (E15: dd15 = dd25)
+  (C11: ur m1 = g0 dd11) (D11: us m2 = g0 dd21)
+  (C13: uq1 m2 = g0 dd13) (D13: ur1 m3 = g0 dd23)
+  (C15: uq1 m1 = g0 dd15) (D15: us m3 = g0 dd25)
+  (E12: hq dd21 = hs dd13) (E14: hq dd11 = hr dd15)
+  (E16: hr dd25 = hs dd23)
+  (HKB1: rew [S0] KB1 in Rr n1 a1 = Rs n2 a2)
+  (HKB3: rew [S0] KB3 in Rq1 n2 a2 = Rr1 n3 a3)
+  (HKB5: rew [S0] KB5 in Rq1 n1 a1 = Rs n3 a3)
+  (HHB1: f_equal ur b1 • (C11 • f_equal g0 E11) =
+         KB1 • (f_equal us b2 • D11))
+  (HHB3: f_equal uq1 b2 • (C13 • f_equal g0 E13) =
+         KB3 • (f_equal ur1 b3 • D13))
+  (HHB5: f_equal uq1 b1 • (C15 • f_equal g0 E15) =
+         KB5 • (f_equal us b3 • D15))
+  (HH2: f_equal fq D11 • (gq dd21 • f_equal f0 E12) =
+        KA2 m2 • (f_equal fs C13 • gs dd13))
+  (HH4: f_equal fq C11 • (gq dd11 • f_equal f0 E14) =
+        KA4 m1 • (f_equal fr C15 • gr dd15))
+  (HH6: f_equal fr D15 • (gr dd25 • f_equal f0 E16) =
+        KA6 m3 • (f_equal fs D13 • gs dd23))
+  (HHA: f_equal fq KB1 • (KA2 n2 • f_equal fs KB3) =
+        KA4 n1 • (f_equal fr KB5 • KA6 n3))
+  (HHs: f_equal hq E11 • (E12 • f_equal hs E13) =
+        E14 • (f_equal hr E15 • E16))
+  (Hcoh2Painting:
+    rew [fun pi: fq (ur n1) = fs (ur1 n3) =>
+        rew [PA] pi in Fq (ur n1) (Rr n1 a1) = Fs (ur1 n3) (Rr1 n3 a3)]
+      HHA in
+    (sigT_map_eq Fq HKB1 ⊙ (HKA2 n2 a2 ⊙ sigT_map_eq Fs HKB3)) =
+    HKA4 n1 a1 ⊙ (sigT_map_eq Fr HKB5 ⊙ HKA6 n3 a3))
+  (Hcoh3Frame: HHA =
+    permutahedral_coherence n1 n2 n3 m1 m2 m3 dd11 dd21 dd13 dd23 dd15 dd25
+      b1 b2 b3 KB1 KB3 KB5 E11 E13 E15 C11 D11 C13 D13 C15 D15 E12 E14 E16
+      HHB1 HHB3 HHB5 HH2 HH4 HH6 HHs):
+  rew [fun pi: hq dd11 = hs dd23 =>
+      rew [fun y => PA (f0 y)] pi in
+      rew [PA] gq dd11 in
+        Fq (g0 dd11) (rew [S0] C11 in Rr m1 (rew [S1] b1 in a1)) =
+      rew [PA] gs dd23 in
+        Fs (g0 dd23) (rew [S0] D13 in Rr1 m3 (rew [S1] b3 in a3))]
+    HHs in
+  (sigT_map_eq (fun x v => rew [PA] gq x in Fq (g0 x) v)
+     (rew_cohLayer S0 g0 Rr Rs E11 b1 b2 C11 D11 KB1 a1 a2 HKB1 HHB1)
+   ⊙ (rew_cohLayer PA f0 Fq Fs E12 D11 C13 (gq dd21) (gs dd13) (KA2 m2)
+        (Rs m2 (rew [S1] b2 in a2)) (Rq1 m2 (rew [S1] b2 in a2))
+        (HKA2 m2 (rew [S1] b2 in a2)) HH2
+      ⊙ sigT_map_eq (fun x v => rew [PA] gs x in Fs (g0 x) v)
+          (rew_cohLayer S0 g0 Rq1 Rr1 E13 b2 b3 C13 D13 KB3 a2 a3
+             HKB3 HHB3))) =
+  rew_cohLayer PA f0 Fq Fr E14 C11 C15 (gq dd11) (gr dd15) (KA4 m1)
+    (Rr m1 (rew [S1] b1 in a1)) (Rq1 m1 (rew [S1] b1 in a1))
+    (HKA4 m1 (rew [S1] b1 in a1)) HH4
+  ⊙ (sigT_map_eq (fun x v => rew [PA] gr x in Fr (g0 x) v)
+       (rew_cohLayer S0 g0 Rq1 Rs E15 b1 b3 C15 D15 KB5 a1 a3 HKB5 HHB5)
+     ⊙ rew_cohLayer PA f0 Fr Fs E16 D15 D13 (gr dd25) (gs dd23) (KA6 m3)
+         (Rs m3 (rew [S1] b3 in a3)) (Rr1 m3 (rew [S1] b3 in a3))
+         (HKA6 m3 (rew [S1] b3 in a3)) HH6).
+Proof.
+  unfold permutahedral_coherence in Hcoh3Frame.
+  destruct b1, b2, b3, E11, E13, E15.
+  lazy beta iota delta [f_equal].
+  change (rew [S1] eq_refl in a1) with a1.
+  change (rew [S1] eq_refl in a2) with a2.
+  change (rew [S1] eq_refl in a3) with a3.
+  cbn in HHB1, HHB3, HHB5, HHs.
+  revert KB1 KB3 KB5 C11 D11 C13 D13 C15 D15 E12 E14 E16 HKB1 HKB3 HKB5
+    HHB1 HHB3 HHB5 HH2 HH4 HH6 HHA HHs Hcoh3Frame Hcoh2Painting.
+  generalize (HKA2 n2 a2). generalize (HKA4 n1 a1). generalize (HKA6 n3 a3).
+  generalize (KA2 n2). generalize (KA4 n1). generalize (KA6 n3).
+  intros k6 k4 k2 hk6 hk4 hk2 KB1 KB3 KB5 C11 D11 C13 D13 C15 D15
+    E12 E14 E16 HKB1 HKB3 HKB5 HHB1 HHB3 HHB5 HH2 HH4 HH6 HHA HHs
+    Hcoh3Frame Hcoh2Painting.
+  rewrite 3 sigT_map_eq_refl.
+  cbv beta.
+  revert KB1 KB3 KB5 D11 D13 D15 C11 C13 C15 HHB1 HHB3 HHB5 HKB1 HKB3 HKB5
+    E16 E12 E14 HHs k2 k4 k6 hk2 hk4 hk6 HH2 HH4 HH6 HHA Hcoh3Frame Hcoh2Painting.
+  generalize (gq dd11). generalize (gs dd13). generalize (gr dd15).
+  cbn.
+  generalize (Rr n1 a1). generalize (Rs n2 a2). generalize (Rq1 n2 a2).
+  generalize (Rr1 n3 a3). generalize (Rq1 n1 a1). generalize (Rs n3 a3).
+  generalize (hq dd11). generalize (hs dd13). generalize (hr dd15).
+  generalize (g0 dd11). generalize (g0 dd13). generalize (g0 dd15).
+  generalize (ur n1). generalize (us n2). generalize (uq1 n2).
+  generalize (ur1 n3). generalize (uq1 n1). generalize (us n3).
+  intros t t0 t1 t2 t3 t4 t5 t6 t7 t8 t9 t10 s s0 s1 s2 s3 s4 ge gs0 gq0
+    KB1 KB3 KB5 D11 D13 D15 C11 C13 C15 HHB1 HHB3 HHB5 HKB1 HKB3 HKB5
+    E16 E12 E14 HHs k2 k4 k6 hk2 hk4 hk6 HH2 HH4 HH6 HHA Hcoh3Frame Hcoh2Painting.
+  revert ge gs0 gq0 C11 C13 C15 HHB1 HHB3 HHB5 HKB1 HKB3 HKB5 E16 E12 E14
+    HHs k2 k4 k6 hk2 hk4 hk6 HH2 HH4 HH6 HHA Hcoh3Frame Hcoh2Painting.
+  destruct D11, D13, D15.
+  intros ge gs0 gq0 C11 C13 C15 HHB1 HHB3 HHB5.
+  cbn in HHB1, HHB3, HHB5.
+  destruct HHB1, HHB3, HHB5.
+  intros HKB1 HKB3 HKB5.
+  destruct HKB1, HKB3, HKB5.
+  revert ge gs0 gq0.
+  destruct C11, C13, C15.
+  intros ge gs0 gq0 E16 E12 E14 HHs.
+  revert E12 E14 HHs ge gs0 gq0.
+  destruct E16.
+  destruct E12.
+  intros E14 HHs. cbn in HHs. destruct HHs.
+  intros ge gs0 gq0.
+  cbn.
+  generalize (Fq t4 s4). generalize (Fs t2 s2). generalize (Fr t0 s0).
+  revert gq0 gs0 ge.
+  generalize (fq t4). generalize (fs t2). generalize (fr t0).
+  intros x x0 x1 gq0 gs0 ge p0 p2 p4 k2 k4 k6 hk2 hk4 hk6
+    HH2 HH4 HH6 HHA Hcoh3Frame Hcoh2Painting.
+  rewrite 3 sigT_trans_eq_refl.
+  revert Hcoh2Painting. revert Hcoh3Frame. revert HH2 HH4 HH6. revert HHA.
+  revert hk2 hk4 hk6. revert k2 k4 k6. revert p0 p2 p4. revert gs0 ge gq0.
+  generalize (f0 t10).
+  destruct gs0.
+  destruct ge.
+  destruct gq0.
+  intros p0 p2 p4 k2 k4 k6 hk2 hk4 hk6 HHA HH2 HH4 HH6 Hcoh3Frame Hcoh2Painting.
+  cbn in HH2, HH4, HH6.
+  revert hk2 hk4 hk6 HHA Hcoh3Frame Hcoh2Painting.
+  destruct HH2, HH4, HH6.
+  intros hk2 hk4.
+  destruct hk2, hk4.
+  intros hk6 HHA Hcoh3Frame Hcoh2Painting.
+  cbn in hk6, HHA, Hcoh3Frame, Hcoh2Painting |- *.
+  rewrite Hcoh3Frame in Hcoh2Painting.
+  cbn in Hcoh2Painting.
+  rewrite 2 sigT_trans_eq_refl in Hcoh2Painting.
+  change (eq_ind p4 (fun p: PA x1 => p4 = p) eq_refl p4 hk6) with (eq_refl • hk6).
+  rewrite eq_trans_refl_l.
+  now exact Hcoh2Painting.
+Defined.
+
+End Coh2Layer.
